resource inference formalisation and proofs (#31)
* ignore append.c which takes too much memory

* ignoring vscode workspace

* Coq changes lost in repo migration

* Normalized `Q` type in `const` (#5)

* use `Qc` type instead of `Q` for rationals in the representation of terms in Coq
* add conversion from `Q` to `Qc` when generating Coq files
* remove useless comment

* Proof of decidable equality

* strengthened simple_resource_inference_step

* add debug messsages to indicate where matching fails

* Stub handling for arrays 

* proof automation: add stub array handling
* add constructor to `log_entry_valid` type to handle arrrays

* cosmetics

* Resource matching checks via `provable`.

* refining resource matching checks

* refactoding and indentation

* debugging aid: print log entry number

* use `subsumed` predicate for `name` in `resource_unfold_struct`

* recursive unfolding

* `struct` and `opaque` constructors for `struct_piece_to_resource`

* cast_ predicate tweaks

* diff for resource unfold

* exists instantiaton

* better exists

* wip

* WIP on re-creating FMap in Ltac2

* solve decidable set equality sub-goals

* require sets to be equal under `ResSet.Equal` in `resource_unfold_full`

* define `is_struct` predicate to make `struct_piece_to_resource` constructors disjoint

* Updates in `CNImpl` module

* declare `CNImpl` as a module with transparent implementation
* don't use `Program Definition` in `CNImpl`
* don't specify `Morello` in compiler details

* logging resource unfolding sub-steps

* Fixes warning from Coq 8.20.1.
closes #4

* update Coq version.
[skip ci]

* removed int field from unfold changed. Reverse log steps

* unused var warning

* Moved predicate_request loging down into mutual recursion

* debugging messages

* fixed CI test problem related to changed line number

* new proof log structure

* tree creation WIP

* missing log entry added

* print number of hints

* indent

* resource folding is now recursive

* tweaking line number to make CI happy

* use `Defined` instead of `Coq` in decidability definitions to make them computable

* functional equivalent of `bt_of_sct_rel` predicate

* proof of equivalence between `bt_of_sct_rel` and `bt_of_sct_fun`

* functional equivalent of `struct_piece_to_resource` predicate

* remove unused parameter in the `struct` constructor of `struct_piece_to_resource` predicate

* proof of equivalence of functional and inductive forms of `struct_piece_to_resource`

* explicit version of `resource_unfold_full` predicate based on the list of intermediate unfolding steps

* subsumed_fun

* work in progress on functional equivalent definitions for `resource_unfold` and `resource_unfold_full`

* resource_unfold_fun

* prove `subsumed_fun_eq`

* define functional equivalent of `resource_unfold_full_explicit`

* printing number of hints for unfold steps

* ambiguous comment removed [skip ci]

* exclude mutual_rec3.c from CI

* change the statement of `resource_unfold_full_explicit_fun_eq` to require the proof in the opposite direction

* comments [skip ci]

* renaming unfold predicates and functions

* fix `unfold_all_explicit_fun` definition

* unfold_step proof with computational reflection

* formatting fix

* perform simplification on resources in hints

* fix OCaml formatting

* performance optimisation

* `struct_piece_to_resource`: move `loc` from predicate arguments to constructor aguments

* use single `struct_loc` value in `struct_piece_to_resource`

* check that the list of fields does not have duplicate ids

* equivalence of `ResSet.In` and `List.In`

* `struct_piece_to_resource` is functional

* `unfold_one_fun_eq`: require the proof only in necessary direction

* prove `unfold_one_fun_eq`

* define `set_from_list` using right fold

* `unfold_all_fixpoint`: input and output can be equal under `ResSet.Equal`

* `unfold_all_explicit_fun`: check that input does not contain structs

* prove `unfold_all_explicit_fun_eq`

* Syle corrections per @cp526 review remarks

---------

Co-authored-by: Valerii Huhnin <33845529+olympichek@users.noreply.github.com>
Co-authored-by: Valerii Huhnin <olympichek1@gmail.com>

lib/pp_mucore_coq.ml
@@ -14,7 +14,7 @@ let pp_Z z =
   if Z.lt z Z.zero then !^("(" ^ s ^ ")%Z") else !^(s ^ "%Z")
 
 
-let pp_Q q = !^("(" ^ Q.to_string q ^ ")%Q")
+let pp_Q q = !^("(" ^ "Q2Qc" ^ "(" ^ Q.to_string q ^ ")%Q)")
 
 (* Prints int as a Coq `nat` *)
 let pp_nat n = !^(string_of_int n)
@@ -2186,24 +2186,31 @@ let pp_context (c : Context.t) =
     ]
 
 
-let pp_resource_inference_type = function
-  | Prooflog.PredicateRequest (s, p, o, ri) ->
+let pp_unpack_result (r : Prooflog.unpack_result) =
+  match r with
+  | Prooflog.UnpackLRT lrt -> pp_constructor "UnpackLRT" [ pp_logical_return_type lrt ]
+  | Prooflog.UnpackRES res -> pp_constructor "UnpackRES" [ pp_list pp_resource res ]
+
+
+let pp_unfold_step (s : Prooflog.unfold_step) =
+  pp_pair (pp_list (pp_pair pp_resource pp_unpack_result)) (pp_list pp_resource) s
+
+
+let rec pp_log_entry = function
+  | Prooflog.PredicateRequest (c, s, p, r, h, c') ->
     pp_constructor
       "PredicateRequest"
-      [ pp_situation s;
+      [ pp_context c;
+        pp_situation s;
         pp_predicate p;
-        pp_option (pp_pair pp_location pp_string) o;
-        pp_pair pp_resource_predicate (pp_list pp_int) ri
+        pp_resource_predicate r;
+        pp_list pp_log_entry h;
+        pp_context c'
       ]
-  | Prooflog.UnfoldResources loc -> pp_constructor "UnfoldResources" [ pp_location loc ]
-
-
-(* Add this definition before its use in `pp_unit_file_with_resource_inference` *)
-let pp_resource_inference_step = function
-  | Prooflog.ResourceInferenceStep (c1, ri, c2) ->
+  | Prooflog.UnfoldResources (c, loc, steps, c') ->
     pp_constructor
-      "ResourceInferenceStep"
-      [ pp_context c1; pp_resource_inference_type ri; pp_context c2 ]
+      "UnfoldResources"
+      [ pp_context c; pp_location loc; pp_list pp_unfold_step steps; pp_context c' ]
 
 
 let coq_steps_var_name = "ResourceInferenceSteps"
@@ -2238,7 +2245,7 @@ let pp_proof_log (steps : Prooflog.log) (generate_proof : bool) =
   ^^ coq_def
        (coq_steps_var_name ^ ":Prooflog.log")
        P.empty
-       (pp_list pp_resource_inference_step steps)
+       (pp_list pp_log_entry (List.rev steps))
   ^^ P.hardline
   ^^
   if generate_proof then
