lib/prooflog.mli
@@ -1,24 +1,31 @@
-type resource_inference_type =
-  | PredicateRequest of
-      Error_common.situation
-      * Request.Predicate.t
-      * (Cerb_location.t * string) option
-      * (Resource.predicate * int list)
-  | UnfoldResources of Cerb_location.t
+type unpack_result =
+  | UnpackLRT of LogicalReturnTypes.t
+  | UnpackRES of Resource.t list
+
+type unfold_changed = (Resource.t * unpack_result) list
+
+type extract_changed = Resource.t list
+
+type unfold_step = unfold_changed * extract_changed
 
 type log_entry =
-  | ResourceInferenceStep of (Context.t * resource_inference_type * Context.t)
+  | PredicateRequest of
+      Context.t
+      * Error_common.situation
+      * Request.Predicate.t
+      * Resource.predicate
+      * log_entry list
+      * Context.t
+  | UnfoldResources of Context.t * Cerb_location.t * unfold_step list * Context.t
 
 type log = log_entry list
 
 val set_enabled : bool -> unit
 
+val is_enabled : unit -> bool
+
 val add_log_entry : log_entry -> unit
 
 val get_proof_log : unit -> log_entry list
 
-val record_resource_inference_step
-  :  Context.t ->
-  Context.t ->
-  resource_inference_type ->
-  unit
+val record_resource_inference_step : log_entry -> unit
