coq/Cn/IndexTerms.v
@@ -6,6 +6,8 @@ Require Import BaseTypes.
 Require Import Terms.
 Require Import Locations.
 
+Import ListNotations.
+
 (* Type aliases *)
 Definition t' := term BaseTypes.t.
 Definition t := annot BaseTypes.t.
@@ -14,21 +16,43 @@ Definition t := annot BaseTypes.t.
 Definition bindings (bt: Type) := list (pattern bt * option (annot bt)).
 Definition t_bindings := bindings BaseTypes.t. 
 
-Module IndexTerm_as_MiniDecidableType <: MiniDecidableType.
-  Definition t := t.
-  Definition eq := @eq t.
-  Lemma eq_dec : forall (x y : t), { eq x y } + { ~ eq x y }.
-  Proof.
-    unfold eq.
-    decide equality; subst.
-    -
-      repeat decide equality.
-    -
-      apply BasetTypes_t_as_MiniDecidableType.eq_dec.
-    -
-      admit.
-  Admitted.
-End IndexTerm_as_MiniDecidableType. 
+Module IndexTerm_as_MiniDecidableType <: MiniDecidableType :=
+  Annot_as_MiniDecidableType BasetTypes_t_as_MiniDecidableType.
 
 Module IndexTerm_as_DecidableType := Make_UDT IndexTerm_as_MiniDecidableType.
 
+(* Defines when a term represents the allocation ID of another term *)
+Inductive eq_ (loc:Locations.t): t -> t -> t -> Prop :=
+| eq_LC: forall t t' bt bt' l l',
+  bt = bt' ->
+    eq_ 
+      loc 
+      (IT _ t bt l) 
+      (IT _ t' bt' l') 
+      (IT _ (Terms.Binop _ Terms.EQ (IT _ t bt l) (IT _ t' bt' l')) (BaseTypes.Bool _) loc).
+
+(* Logical relation that defines when a list of terms represents equality between two lists *)
+Inductive eq_list_rel (loc: Locations.t) : list t -> list t -> list t -> Prop :=
+| eq_list_nil: 
+    eq_list_rel loc [] [] []
+| eq_list_cons: forall x y xs ys eq_terms eq_term,
+    eq_ loc x y eq_term ->
+    eq_list_rel loc xs ys eq_terms ->
+    eq_list_rel loc (x :: xs) (y :: ys) (eq_term :: eq_terms).
+
+Definition and2_ (loc: Locations.t) (t1 t2: t) :=
+  IT _ (Terms.Binop _ Terms.And t1 t2) (BaseTypes.Bool _) loc.
+
+Inductive and_ (loc: Locations.t) : list t -> t -> Prop :=
+| and_nil: and_ loc [] (IT _ (Terms.Const _ (Terms.Bool true)) (BaseTypes.Bool _) loc)
+| and_singleton: forall t, and_ loc [t] t
+| and_cons: forall t ts result_t,
+    and_ loc ts result_t ->
+    and_ loc (t :: ts) (and2_ loc t result_t).
+
+(* Logical relation that defines when a term represents the conjunction of equalities between two lists *)
+Inductive eq_and_list_rel (loc: Locations.t) : list t -> list t -> t -> Prop :=
+| eq_and_list_rel_intro: forall xs ys eq_terms conj_term,
+    eq_list_rel loc xs ys eq_terms ->
+    and_ loc eq_terms conj_term ->
+    eq_and_list_rel loc xs ys conj_term. 
