coq/Cn/Resource.v
@@ -14,25 +14,52 @@ Definition qpredicate : Type := Request.QPredicate.t * output.
 
 Definition t : Type := Request.t * output.
 
+Module Output_as_MiniDecidableType <: MiniDecidableType.
+  Definition t := output.
+  Definition eq := @eq t.
+  Lemma eq_dec : forall (x y : t), { eq x y } + { ~ eq x y }.
+  Proof.
+    unfold eq.
+    intros [o1] [o2].
+    decide equality.
+    apply IndexTerm_as_MiniDecidableType.eq_dec.
+  Defined.
+End Output_as_MiniDecidableType.
+
 Module Resource_as_MiniDecidableType <: MiniDecidableType.
   Definition t := t.
   Definition eq := @eq t.
   Lemma eq_dec : forall (x y : t), { eq x y } + { ~ eq x y }.
   Proof.
-    unfold eq.
-    decide equality.
-    -
-      subst.
-      decide equality.
-      apply IndexTerm_as_MiniDecidableType.eq_dec.
-    -
-      admit.
-  Admitted.
+    intros r1 r2.
+    apply BaseTypes.prod_eq_dec.
+    - apply Request_as_MiniDecidableType.eq_dec.
+    - apply Output_as_MiniDecidableType.eq_dec.
+  Defined.
 End Resource_as_MiniDecidableType.
 
+Module Output_as_DecidableType := Make_UDT Output_as_MiniDecidableType.
 Module Resource_as_DecidableType := Make_UDT Resource_as_MiniDecidableType.
 Module ResSet := FSetWeakList.Make Resource_as_DecidableType.
 Module ResSetDecide := FSetDecide.WDecide(ResSet).
 
 Definition set_from_list (l : list t) : ResSet.t :=
-  List.fold_left (fun s c => ResSet.add c s) l ResSet.empty.
+  List.fold_right (fun c s => ResSet.add c s) ResSet.empty l.
+
+Lemma ResSet_In_List_In_eq: forall r rs,
+  ResSet.In r (Resource.set_from_list rs) <-> List.In r rs.
+Proof.
+  intros r rs.
+  induction rs.
+  { split; intros H; inversion H. }
+  cbn.
+  split; intros H.
+  - apply ResSetDecide.F.add_iff in H.
+    destruct H as [H | H].
+    + left; apply H.
+    + right; apply IHrs, H.
+  - apply ResSetDecide.F.add_iff.
+    destruct H as [H | H].
+    + left; apply H.
+    + right; apply IHrs, H.
+Qed.
