coq/Cn/SCtypes.v
@@ -1,10 +1,16 @@
+Require Import Coq.Structures.DecidableType.
+Require Import Coq.Structures.DecidableTypeEx.
+Require Import Coq.Program.Equality.
 Require Import Cerberus.Symbol.
 Require Import Cerberus.IntegerType.
 Require Import Cerberus.Ctype.
+Require Import Sym.
+Require Import BaseTypes.
 (* Qualifiers *)
 Definition qualifiers := Ctype.qualifiers.
 
 (* C types *)
+Unset Elimination Schemes.
 Inductive ctype : Type :=
   | Void : ctype
   | Integer : integerType -> ctype
@@ -12,6 +18,39 @@ Inductive ctype : Type :=
   | Pointer : ctype -> ctype
   | Struct : sym -> ctype
   | SCFunction : (qualifiers * ctype) * (list (ctype * bool)) * bool -> ctype.
+Set Elimination Schemes.
+
+(* We define a custom induction principle for [ctype] because the
+   default one incorrectly handles hidden recursive cases for the
+   [Array] and [SCFunction] constructors. *)
+Theorem ctype_ind_set (P : ctype -> Type):
+  P Void ->
+  (forall i : integerType, P (Integer i)) ->
+  (forall p : ctype * option nat, P (fst p) -> P (Array p)) ->
+  (forall c : ctype, P c -> P (Pointer c)) ->
+  (forall s : sym, P (Struct s)) ->
+  (forall p : qualifiers * ctype * list (ctype * bool) * bool,
+    P (snd (fst (fst p))) ->
+    Forall_type (fun '(x, _) => P x) (snd (fst p)) -> 
+    P (SCFunction p))
+  -> forall t : ctype, P t.
+Proof.
+  intros HVoid HInteger HArray HPointer HStruct HSCFunction.
+  fix IH 1.
+  intros t.
+  destruct t.
+  - apply HVoid.
+  - apply HInteger.
+  - apply HArray, IH.
+  - apply HPointer, IH.
+  - apply HStruct.
+  - apply HSCFunction.
+    + apply IH.
+    + destruct p as [[[q c] l] b].
+      induction l as [| [c' b'] l IHl].
+      * constructor.
+      * constructor; auto.
+Defined.
 
 Definition t := ctype.
 
@@ -29,3 +68,103 @@ Record c_concrete_sig := mk_c_concrete_sig {
   sig_variadic : bool;
   sig_has_proto : bool
 }.
+
+Module IntegerBaseType_as_MiniDecidableType <: MiniDecidableType.
+  Definition t := integerBaseType.
+  Definition eq := @eq t.
+  Lemma eq_dec : forall (x y : t), { eq x y } + { ~ eq x y }.
+  Proof.
+    unfold eq.
+    intros x y.
+    destruct x, y.
+    all: try (right; discriminate).
+    all: try (left; reflexivity).
+    all: decide equality.
+    all: apply Nat_as_DT.eq_dec.
+  Defined.
+End IntegerBaseType_as_MiniDecidableType.
+
+Module IntegerType_as_MiniDecidableType <: MiniDecidableType.
+  Definition t := integerType.
+  Definition eq := @eq t.
+  Lemma eq_dec : forall (x y : t), { eq x y } + { ~ eq x y }.
+  Proof.
+    unfold eq.
+    intros x y.
+    destruct x, y.
+    all: try (right; discriminate).
+    all: try (left; reflexivity).
+    all: decide equality.
+    all: try apply IntegerBaseType_as_MiniDecidableType.eq_dec.
+    all: try apply Sym_t_as_MiniDecidableType.eq_dec.
+  Defined.
+End IntegerType_as_MiniDecidableType.
+
+Module qualifiers_as_MiniDecidableType <: MiniDecidableType.
+  Definition t := qualifiers.
+  Definition eq := @eq t.
+  Lemma eq_dec : forall (x y : t), { eq x y } + { ~ eq x y }.
+  Proof.
+    unfold eq.
+    intros x y.
+    destruct x, y.
+    do 2 decide equality.
+  Defined.
+End qualifiers_as_MiniDecidableType.
+
+Module SCtypes_as_MiniDecidableType <: MiniDecidableType.
+  Definition t := t.
+  Definition eq := @eq t.
+  Lemma eq_dec : forall (x y : t), { eq x y } + { ~ eq x y }.
+  Proof.
+    unfold eq.
+    apply (ctype_ind_set (fun x => forall y, { x = y } + { x <> y })).
+    - intros y.
+      destruct y; try (right; discriminate).
+      left; reflexivity.
+    - intros i y.
+      destruct y; try (right; discriminate).
+      destruct (IntegerType_as_MiniDecidableType.eq_dec i i0) as [E | NE]; try (right; congruence).
+      inversion E; subst.
+      left; reflexivity.
+    - intros [x n] IH y.
+      destruct y; try (right; discriminate).
+      destruct p as [x' n'].
+      cbn in IH.      
+      destruct (IH x') as [E | NE]; try (right; congruence); subst.
+      destruct (option_eq_dec Nat_as_DT.eq_dec n n') as [En | NEn]; try (right; congruence); subst.
+      left; reflexivity.
+    - intros x IH y.
+      destruct y; try (right; discriminate).
+      destruct (IH y) as [E | NE]; try (right; congruence); subst.
+      left; reflexivity.
+    - intros s x.
+      destruct x; try (right; discriminate).
+      destruct (Sym_t_as_MiniDecidableType.eq_dec s s0) as [Es | NEs]; try (right; congruence).
+      inversion Es; subst.
+      left; reflexivity.
+    - intros [[[q x] l] b] IH IHl y.
+      destruct y; try (right; discriminate).
+      destruct p as [[[q' x'] l'] b'].
+      cbn in *.
+      revert l'.
+      induction IHl as [| [x1 b1] l IH' _ IHl]; intros l'.
+      + destruct l'; try (right; discriminate).
+        destruct (qualifiers_as_MiniDecidableType.eq_dec q q') as [Eq | NEq]; try (right; congruence).
+        inversion Eq; subst.
+        destruct (IH x') as [E | NE]; try (right; congruence); subst.
+        destruct (Bool.bool_dec b b') as [Eb | NEb]; try (right; congruence); subst.
+        left; reflexivity.
+      + destruct l'; try (right; discriminate).
+        destruct p as [x1' b1'].
+        destruct (qualifiers_as_MiniDecidableType.eq_dec q q') as [Eq | NEq]; try (right; congruence).
+        inversion Eq; subst.
+        destruct (IH x') as [E | NE]; try (right; congruence); subst.
+        destruct (Bool.bool_dec b b') as [Eb | NEb]; try (right; congruence); subst.
+        destruct (IH' x1') as [E | NE]; try (right; congruence); subst.
+        destruct (Bool.bool_dec b1 b1') as [Eb1 | NEb1]; try (right; congruence); subst.
+        destruct (IHl l') as [E | NE]; try (right; congruence).
+        inversion E; subst.
+        left; reflexivity.
+  Defined.
+End SCtypes_as_MiniDecidableType.
