coq/Cn/Terms.v
@@ -1,8 +1,12 @@
 Require Import ZArith.
 Require Import String.
 Require Import List.
-Require Import QArith.
+Require Import QArith.Qcanon.
+Require Import List.
+Require Import Coq.Structures.DecidableType.
+Require Import Coq.Structures.DecidableTypeEx.
 Require Import Cerberus.Symbol.
+Require Import Sym.
 Require Import BaseTypes.
 Require Import Cerberus.Location.
 Require Import SCtypes.
@@ -13,7 +17,7 @@ Require Import Cerberus.IntegerType.
 Inductive const : Type :=
   | Z : Z -> const
   | Bits : (BaseTypes.sign * nat) * Z -> const
-  | Q : Q -> const  (* Note: Q needs to be defined or imported *)
+  | Q : Qc -> const
   | MemByte : Z * Z -> const  (* alloc_id * value *)
   | Pointer : Z * Z -> const  (* alloc_id * addr *)
   | Alloc_id : Z -> const
@@ -68,6 +72,8 @@ Inductive binop : Type :=
   | SetMember : binop
   | Subset : binop.
 
+Unset Elimination Schemes.
+
 (* Patterns *)
 Inductive pattern_ (bt : Type) : Type :=
   | PSym : sym -> pattern_ bt
@@ -121,3 +127,680 @@ Inductive term (bt : Type) : Type :=
 
 with annot (bt : Type) : Type :=
   | IT : term bt -> bt -> Locations.t -> annot bt.
+
+Set Elimination Schemes.
+
+(* We define a custom induction principle for [pattern_] to properly handle
+   mutual induction and constructors with hidden recursive cases. *)
+Theorem pattern__ind_set (ty : Type) (P : pattern_ ty -> Type) (P' : pattern ty -> Type) :
+  (forall (s : sym), P (PSym ty s)) ->
+  (P (PWild ty)) ->
+  (forall (s : sym) (l : list (Symbol.identifier * pattern ty)),
+    Forall_type (fun '(_, p) => P' p) l -> P (PConstructor ty s l)) ->
+  (forall (p : pattern_ ty) (tt : ty) (lc : Locations.t), P p -> P' (Pat ty p tt lc)) ->
+  forall p : pattern_ ty, P p.
+Proof.
+  intros HPSym HPWild HPConstructor HPPat.
+  fix IH 1.
+  intros p.
+  destruct p.
+  - apply HPSym.
+  - apply HPWild.
+  - clear - HPConstructor HPPat IH.
+    apply HPConstructor.
+    induction l.
+    + apply Forall_nil.
+    + destruct a as [i p].
+      destruct p.
+      apply Forall_cons.
+      * apply HPPat, IH.
+      * apply IHl.
+Qed.
+
+(* We define a custom induction principle for [term] to properly handle
+   mutual induction and constructors with hidden recursive cases. *)
+Theorem term_ind_set (ty : Type) (P : term ty -> Type) (P' : annot ty -> Type) :
+  (forall (c : const), P (Const ty c)) ->
+  (forall (s : sym), P (Sym ty s)) ->
+  (forall (u : unop) (a : annot ty), P' a -> P (Unop ty u a)) ->
+  (forall (b : binop) (a1 a2 : annot ty), P' a1 -> P' a2 -> P (Binop ty b a1 a2)) ->
+  (forall (a1 a2 a3 : annot ty), P' a1 -> P' a2 -> P' a3 -> P (ITE ty a1 a2 a3)) ->
+  (forall (p : nat * (sym * BaseTypes.t) * nat) (a : annot ty), P' a -> P (EachI ty p a)) ->
+  (forall (l : list (annot ty)), Forall_type (fun a => P' a) l -> P (Tuple ty l)) ->
+  (forall (n : nat) (a : annot ty), P' a -> P (NthTuple ty n a)) ->
+  (forall (s : sym) (l : list (identifier * annot ty)), Forall_type (fun '(_, a) => P' a) l -> P (Struct ty s l)) ->
+  (forall (a : annot ty) (i : identifier), P' a -> P (StructMember ty a i)) ->
+  (forall (p : annot ty * identifier) (a : annot ty), P' (fst p) -> P' a -> P (StructUpdate ty p a)) ->
+  (forall (l : list (identifier * annot ty)), Forall_type (fun '(_, a) => P' a) l -> P (TRecord ty l)) ->
+  (forall (a : annot ty) (i : identifier), P' a -> P (RecordMember ty a i)) ->
+  (forall (p : annot ty * identifier) (a : annot ty), P' (fst p) -> P' a -> P (RecordUpdate ty p a)) ->
+  (forall (s : sym) (l : list (identifier * annot ty)), Forall_type (fun '(_, a) => P' a) l -> P (Constructor ty s l)) ->
+  (forall (a : annot ty) (s : sym) (i : identifier), P' a -> P (MemberShift ty a s i)) ->
+  (forall (a1 : annot ty) (ct : SCtypes.t) (a2 : annot ty), P' a1 -> P' a2 -> P (ArrayShift ty a1 ct a2)) ->
+  (forall (a1 a2 : annot ty), P' a1 -> P' a2 -> P (CopyAllocId ty a1 a2)) ->
+  (forall (a : annot ty), P' a -> P (HasAllocId ty a)) ->
+  (forall (ct : SCtypes.t), P (SizeOf ty ct)) ->
+  (forall (s : sym) (i : identifier), P (OffsetOf ty s i)) ->
+  (forall (bt : BaseTypes.t), P (Nil ty bt)) ->
+  (forall (a1 a2 : annot ty), P' a1 -> P' a2 -> P (Cons ty a1 a2)) ->
+  (forall (a : annot ty), P' a -> P (Head ty a)) ->
+  (forall (a : annot ty), P' a -> P (Tail ty a)) ->
+  (forall (a1 a2 a3 : annot ty), P' a1 -> P' a2 -> P' a3 -> P (NthList ty a1 a2 a3)) ->
+  (forall (a1 a2 a3: annot ty), P' a1 -> P' a2 -> P' a3 -> P (ArrayToList ty a1 a2 a3)) ->
+  (forall (ct : SCtypes.t) (a : annot ty) , P' a -> P (Representable ty ct a)) ->
+  (forall (ct : SCtypes.t) (a : annot ty) , P' a -> P (Good ty ct a)) ->
+  (forall (a1 a2 : annot ty), P' a1 -> P' a2 -> P (Aligned ty a1 a2)) ->
+  (forall (i : IntegerType.t) (a : annot ty), P' a -> P (WrapI ty i a)) ->
+  (forall (bt : BaseTypes.t) (a : annot ty), P' a -> P (MapConst ty bt a)) ->
+  (forall (a1 a2 a3 : annot ty), P' a1 -> P' a2 -> P' a3 -> P (MapSet ty a1 a2 a3)) ->
+  (forall (a1 a2 : annot ty), P' a1 -> P' a2 -> P (MapGet ty a1 a2)) ->
+  (forall (p : sym * BaseTypes.t) (a : annot ty), P' a -> P (MapDef ty p a)) ->
+  (forall (s : sym) (l : list (annot ty)), Forall_type (fun a => P' a) l -> P (Apply ty s l)) ->
+  (forall (p : sym * annot ty) (a : annot ty), P' (snd p) -> P' a -> P (TLet ty p a)) ->
+  (forall (a : annot ty) (l : list (pattern ty * annot ty)), P' a -> Forall_type (fun '(_, a) => P' a) l -> P (TMatch ty a l)) ->
+  (forall (bt : BaseTypes.t) (a : annot ty), P' a -> P (Cast ty bt a)) ->
+  (forall (t : term ty) (tt : ty) (lc : Locations.t), P t -> P' (IT ty t tt lc)) ->
+  forall t : term ty, P t.
+Proof.
+  intros HConst HSym HUnop HBinop HITE HEachI HTuple HNthTuple HStruct
+         HStructMember HStructUpdate HTRecord HRecordMember HRecordUpdate
+         HConstructor HMemberShift HArrayShift HCopyAllocId HHasAllocId
+         HSizeOf HOffsetOf HNil HCons HHead HTail HNthList HArrayToList
+         HRepresentable HGood HAligned HWrapI HMapConst HMapSet HMapGet
+         HMapDef HApply HTLet HTMatch HCast HIT.
+  fix IH 1.
+  intros t.
+  destruct t.
+  - apply HConst.
+  - apply HSym.
+  - clear - HUnop HIT IH.
+    destruct a.
+    apply HUnop, HIT, IH.
+  - clear - HBinop HIT IH.
+    destruct a, a0.
+    apply HBinop; apply HIT, IH.
+  - clear - HITE HIT IH.
+    destruct a, a0, a1.
+    apply HITE; apply HIT, IH.
+  - clear - HEachI HIT IH.
+    destruct a.
+    apply HEachI, HIT, IH.
+  - clear - HTuple HIT IH.
+    apply HTuple.
+    induction l.
+    + apply Forall_nil.
+    + destruct a.
+      apply Forall_cons.
+      * apply HIT, IH.
+      * apply IHl.
+  - clear - HNthTuple HIT IH.
+    destruct a.
+    apply HNthTuple, HIT, IH.
+  - clear - HStruct HIT IH.
+    apply HStruct.
+    induction l.
+    + apply Forall_nil.
+    + destruct a as [? a], a.
+      apply Forall_cons.
+      * apply HIT, IH.
+      * apply IHl.
+  - clear - HStructMember HIT IH.
+    destruct a.
+    apply HStructMember, HIT, IH.
+  - clear - HStructUpdate HIT IH.
+    destruct a, p as [a1 ?], a1.
+    apply HStructUpdate; apply HIT, IH.
+  - clear - HTRecord HIT IH.
+    apply HTRecord.
+    induction l.
+    + apply Forall_nil.
+    + destruct a as [? a], a.
+      apply Forall_cons.
+      * apply HIT, IH.
+      * apply IHl.
+  - clear - HRecordMember HIT IH.
+    destruct a.
+    apply HRecordMember, HIT, IH.
+  - clear - HRecordUpdate HIT IH.
+    destruct a, p as [a1 ?], a1.
+    apply HRecordUpdate; apply HIT, IH.
+  - clear - HConstructor HIT IH.
+    apply HConstructor.
+    induction l.
+    + apply Forall_nil.
+    + destruct a as [? a], a.
+      apply Forall_cons.
+      * apply HIT, IH.
+      * apply IHl.
+  - clear - HMemberShift HIT IH.
+    destruct a.
+    apply HMemberShift; apply HIT, IH.
+  - clear - HArrayShift HIT IH.
+    destruct a, a0.
+    apply HArrayShift; apply HIT, IH.
+  - clear - HCopyAllocId HIT IH.
+    destruct a, a0.
+    apply HCopyAllocId; apply HIT, IH.
+  - clear - HHasAllocId HIT IH.
+    destruct a.
+    apply HHasAllocId; apply HIT, IH.
+  - apply HSizeOf.
+  - apply HOffsetOf.
+  - apply HNil.
+  - clear - HCons HIT IH.
+    destruct a, a0.
+    apply HCons; apply HIT, IH.
+  - clear - HHead HIT IH.
+    destruct a.
+    apply HHead; apply HIT, IH.
+  - clear - HTail HIT IH.
+    destruct a.
+    apply HTail; apply HIT, IH.
+  - clear - HNthList HIT IH.
+    destruct a, a0, a1.
+    apply HNthList; apply HIT, IH.
+  - clear - HArrayToList HIT IH.
+    destruct a, a0, a1.
+    apply HArrayToList; apply HIT, IH.
+  - clear - HRepresentable HIT IH.
+    destruct a.
+    apply HRepresentable, HIT, IH.
+  - clear - HGood HIT IH.
+    destruct a.
+    apply HGood, HIT, IH.
+  - clear - HAligned HIT IH.
+    destruct a, a0.
+    apply HAligned; apply HIT, IH.
+  - clear - HWrapI HIT IH.
+    destruct a.
+    apply HWrapI, HIT, IH.
+  - clear - HMapConst HIT IH.
+    destruct a.
+    apply HMapConst, HIT, IH.
+  - clear - HMapSet HIT IH.
+    destruct a, a0, a1.
+    apply HMapSet; apply HIT, IH.
+  - clear - HMapGet HIT IH.
+    destruct a, a0.
+    apply HMapGet; apply HIT, IH.
+  - clear - HMapDef HIT IH.
+    destruct a.
+    apply HMapDef, HIT, IH.
+  - clear - HApply HIT IH.
+    apply HApply.
+    induction l.
+    + apply Forall_nil.
+    + destruct a.
+      apply Forall_cons.
+      * apply HIT, IH.
+      * apply IHl.
+  - clear - HTLet HIT IH.
+    destruct a, p as [? a], a.
+    apply HTLet; apply HIT, IH.
+  - clear - HTMatch HIT IH.
+    destruct a.
+    apply HTMatch.
+    + apply HIT, IH.
+    + induction l.
+      * apply Forall_nil.
+      * destruct a as [? a], a.
+        apply Forall_cons.
+        -- apply HIT, IH.
+        -- apply IHl.
+  - clear - HCast HIT IH.
+    destruct a.
+    apply HCast; apply HIT, IH.
+Defined.
+
+Module Const_as_MiniDecidableType <: MiniDecidableType.
+  Definition t := const.
+  Definition eq := @eq t.
+  Lemma eq_dec : forall (x y : t), { eq x y } + { ~ eq x y }.
+  Proof.
+    unfold eq.
+    intros x y.
+    destruct x, y; try (right; discriminate).
+    - destruct (Z_as_DT.eq_dec z z0); try (right; congruence); subst.
+      left; reflexivity.
+    - destruct p as [[s n] z], p0 as [[s' n'] z'].
+      destruct (Nat_as_DT.eq_dec n n'); try (right; congruence); subst.
+      destruct (sign_eq_dec s s'); try (right; congruence); subst.
+      destruct (Z_as_DT.eq_dec z z'); try (right; congruence); subst.
+      left; reflexivity.
+    - destruct (Qc_eq_dec q q0); try (right; congruence); subst.
+      left; reflexivity.
+    - destruct p as [z1 z2], p0 as [z1' z2'].
+      destruct (Z_as_DT.eq_dec z1 z1'); try (right; congruence); subst.
+      destruct (Z_as_DT.eq_dec z2 z2'); try (right; congruence); subst.
+      left; reflexivity.
+    - destruct p as [z1 z2], p0 as [z1' z2'].
+      destruct (Z_as_DT.eq_dec z1 z1'); try (right; congruence); subst.
+      destruct (Z_as_DT.eq_dec z2 z2'); try (right; congruence); subst.
+      left; reflexivity.
+    - destruct (Z_as_DT.eq_dec z z0); try (right; congruence); subst.
+      left; reflexivity.
+    - destruct (Bool.bool_dec b b0); try (right; congruence); subst.
+      left; reflexivity.
+    - left; reflexivity.
+    - left; reflexivity.
+    - destruct (SCtypes_as_MiniDecidableType.eq_dec c c0) as [E | NE]; try (right; congruence).
+      inversion E; subst; left; reflexivity.
+    - destruct (BasetTypes_t_as_MiniDecidableType.eq_dec t0 t1) as [E | NE]; try (right; congruence).
+      inversion E; subst; left; reflexivity.
+  Defined.
+End Const_as_MiniDecidableType.
+
+Module Unop_as_MiniDecidableType <: MiniDecidableType.
+  Definition t := unop.
+  Definition eq := @eq t.
+  Lemma eq_dec : forall (x y : t), { eq x y } + { ~ eq x y }.
+  Proof.
+    unfold eq.
+    decide equality.
+  Defined.
+End Unop_as_MiniDecidableType.
+
+Module Binop_as_MiniDecidableType <: MiniDecidableType.
+  Definition t := binop.
+  Definition eq := @eq t.
+  Lemma eq_dec : forall (x y : t), { eq x y } + { ~ eq x y }.
+  Proof.
+    unfold eq.
+    decide equality.
+  Defined.
+End Binop_as_MiniDecidableType.
+
+Module Pattern__as_MiniDecidableType (Ty_as_MiniDecidableType : MiniDecidableType) <: MiniDecidableType.
+  Definition ty := Ty_as_MiniDecidableType.t.
+
+  Lemma eq_dec : forall (x y : pattern_ ty), { eq x y } + { ~ eq x y }.
+  Proof.
+    apply (pattern__ind_set ty
+      (fun p1 => forall p2, { eq p1 p2 } + { ~ eq p1 p2 })
+      (fun p1 => forall p2, { eq p1 p2 } + { ~ eq p1 p2 })).
+    - intros s p0.
+      destruct p0; try (right; discriminate).
+      destruct (Sym_t_as_MiniDecidableType.eq_dec s s0) as [E | ?]; try (right; congruence).
+      inversion E; subst; left; reflexivity.
+    - intros p0.
+      destruct p0; try (right; discriminate).
+      left; reflexivity.
+    - intros s l IHl p0.
+      destruct p0; try (right; discriminate).
+      destruct (Sym_t_as_MiniDecidableType.eq_dec s s0) as [E | ?]; try (right; congruence).
+      inversion E; subst; clear E.
+      revert l0.
+      induction IHl as [| [i p] l IHp _ IHl]; intros l0.
+      + destruct l0; try (right; discriminate).
+        left; reflexivity.
+      + destruct l0; try (right; discriminate).
+        destruct p0 as [i0 p0].
+        destruct (Symbol_identifier_as_MiniDecidableType.eq_dec i i0) as [E | ?]; try (right; congruence).
+        inversion E; subst; clear E.
+        destruct (IHp p0) as [E | ?]; try (right; congruence); subst.
+        destruct (IHl l0) as [E | ?]; try (right; congruence).
+        inversion E; subst; clear E.
+        left; reflexivity.
+    - intros p tt lc IHp p0.
+      destruct p0; try (right; discriminate).
+      destruct (Locations_t_as_MiniDecidableType.eq_dec lc t0) as [E | ?]; try (right; congruence).
+      inversion E; subst; clear E.
+      destruct (Ty_as_MiniDecidableType.eq_dec tt t) as [E | ?]; try (right; congruence); subst.
+      destruct (IHp p0); try (right; congruence); subst.
+      left; reflexivity.
+  Defined.
+
+  Definition t := pattern_ ty.
+  Definition eq := @eq t.
+End Pattern__as_MiniDecidableType.
+
+Module Pattern_as_MiniDecidableType (Ty_as_MiniDecidableType : MiniDecidableType) <: MiniDecidableType.
+  Module Pattern__as_MiniDecidableType := Pattern__as_MiniDecidableType Ty_as_MiniDecidableType.
+  Definition ty := Ty_as_MiniDecidableType.t.
+  Definition t := pattern ty.
+  Definition eq := @eq t.
+  Lemma eq_dec : forall (x y : t), { eq x y } + { ~ eq x y }.
+  Proof.
+    unfold eq.
+    intros [p1 tt1 lc1] [p2 tt2 lc2].
+    destruct (Pattern__as_MiniDecidableType.eq_dec p1 p2); try (right; congruence); subst.
+    destruct (Ty_as_MiniDecidableType.eq_dec tt1 tt2); try (right; congruence); subst.
+    destruct (Locations_t_as_MiniDecidableType.eq_dec lc1 lc2) as [E | NE]; try (right; congruence).
+    inversion E; subst; left; reflexivity.
+  Defined.
+End Pattern_as_MiniDecidableType.
+
+Module Term_as_MiniDecidableType (Ty_as_MiniDecidableType : MiniDecidableType) <: MiniDecidableType.
+  Module Pattern_as_MiniDecidableType := Pattern_as_MiniDecidableType Ty_as_MiniDecidableType.
+  Definition ty := Ty_as_MiniDecidableType.t.
+
+  Lemma eq_dec : forall (x y : term ty), { eq x y } + { ~ eq x y }.
+  Proof.
+    apply (term_ind_set ty
+            (fun t1 => forall t2, { eq t1 t2 } + { ~ eq t1 t2 })
+            (fun a1 => forall a2, { eq a1 a2 } + { ~ eq a1 a2 })).
+    - intros c t0.
+      destruct t0; try (right; discriminate).
+      destruct (Const_as_MiniDecidableType.eq_dec c c0) as [E | ?]; try (right; congruence).
+      inversion E; subst; left; reflexivity.
+    - intros s t0.
+      destruct t0; try (right; discriminate).
+      destruct (Sym_t_as_MiniDecidableType.eq_dec s s0) as [E | ?]; try (right; congruence).
+      inversion E; subst; left; reflexivity.
+    - intros u a IHa t0.
+      destruct t0; try (right; discriminate).
+      destruct (Unop_as_MiniDecidableType.eq_dec u u0) as [E | ?]; try (right; congruence).
+      inversion E; subst; clear E.
+      destruct (IHa a0); try (right; congruence); subst.
+      left; reflexivity.
+    - intros b a1 a2 IHa1 IHa2 t0.
+      destruct t0; try (right; discriminate).
+      destruct (Binop_as_MiniDecidableType.eq_dec b b0) as [E | ?]; try (right; congruence).
+      inversion E; subst; clear E.
+      destruct (IHa1 a); try (right; congruence); subst.
+      destruct (IHa2 a0); try (right; congruence); subst.
+      left; reflexivity.
+    - intros a1 a2 a3 IHa1 IHa2 IHa3 t0.
+      destruct t0; try (right; discriminate).
+      destruct (IHa1 a); try (right; congruence); subst.
+      destruct (IHa2 a0); try (right; congruence); subst.
+      destruct (IHa3 a4); try (right; congruence); subst.
+      left; reflexivity.
+    - intros p a IHa t0.
+      destruct t0; try (right; discriminate).
+      destruct p as [[n1 [s bt]] n2].
+      destruct p0 as [[n1' [s' bt']] n2'].
+      destruct (Nat_as_DT.eq_dec n1 n1'); try (right; congruence).
+      destruct (Sym_t_as_MiniDecidableType.eq_dec s s') as [E | ?]; try (right; congruence).
+      inversion E; subst; clear E.
+      destruct (BasetTypes_t_as_MiniDecidableType.eq_dec bt bt') as [E | ?]; try (right; congruence).
+      inversion E; subst; clear E.
+      destruct (Nat_as_DT.eq_dec n2 n2'); try (right; congruence); subst.
+      destruct (IHa a0); try (right; congruence); subst.
+      left; reflexivity.
+    - intros l IHl t0.
+      destruct t0; try (right; discriminate).
+      revert l0.
+      induction IHl as [| [t tt] l IH _ IHl]; intros l0.
+      + destruct l0; try (right; discriminate).
+        left; reflexivity.
+      + destruct l0; try (right; discriminate).
+        destruct (IH a) as [E | ?]; try (right; congruence).
+        destruct a.
+        inversion E; subst; clear E.
+        destruct (IHl l0) as [E | ?]; try (right; congruence).
+        inversion E; subst; clear E.
+        left; reflexivity.
+    - intros n a IHa t0.
+      destruct t0; try (right; discriminate).
+      destruct (Nat_as_DT.eq_dec n n0); try (right; congruence); subst.
+      destruct (IHa a0); try (right; congruence); subst.
+      left; reflexivity.
+    - intros s l IHl t0.
+      destruct t0; try (right; discriminate).
+      destruct (Sym_t_as_MiniDecidableType.eq_dec s s0) as [E | ?]; try (right; congruence).
+      inversion E; subst; clear E.
+      revert l0.
+      induction IHl as [| [i a] l IHa _ IHl]; intros l0.
+      + destruct l0; try (right; discriminate).
+        left; reflexivity.
+      + destruct l0; try (right; discriminate).
+        destruct p as [i0 a0].
+        destruct (Symbol_identifier_as_MiniDecidableType.eq_dec i i0) as [E | ?]; try (right; congruence).
+        inversion E; subst; clear E.
+        destruct (IHa a0) as [E | ?]; try (right; congruence); subst.
+        destruct (IHl l0) as [E | ?]; try (right; congruence).
+        inversion E; subst; clear E.
+        left; reflexivity.
+    - intros a i IHa t0. 
+      destruct t0; try (right; discriminate).
+      destruct (Symbol_identifier_as_MiniDecidableType.eq_dec i i0) as [E | ?]; try (right; congruence).
+      inversion E; subst; clear E.
+      destruct (IHa a0); try (right; congruence); subst.
+      left; reflexivity.
+    - intros p a1 IHa2 IHa1 t0.
+      destruct t0; try (right; discriminate).
+      destruct p as [a2 i].
+      destruct p0 as [a2' i'].
+      destruct (Symbol_identifier_as_MiniDecidableType.eq_dec i i') as [E | ?]; try (right; congruence).
+      inversion E; subst; clear E.
+      cbn in *.
+      destruct (IHa2 a2'); try (right; congruence); subst.
+      destruct (IHa1 a); try (right; congruence); subst.
+      left; reflexivity.
+    - intros l IHl t0.
+      destruct t0; try (right; discriminate).
+      revert l0.
+      induction IHl as [| [i a] l IHa _ IHl]; intros l0.
+      + destruct l0; try (right; discriminate).
+        left; reflexivity.
+      + destruct l0; try (right; discriminate).
+        destruct p as [i0 a0].
+        destruct (Symbol_identifier_as_MiniDecidableType.eq_dec i i0) as [E | ?]; try (right; congruence).
+        inversion E; subst; clear E.
+        destruct (IHa a0) as [E | ?]; try (right; congruence); subst.
+        destruct (IHl l0) as [E | ?]; try (right; congruence).
+        inversion E; subst; clear E.
+        left; reflexivity.
+    - intros a i IHa t0.
+      destruct t0; try (right; discriminate).
+      destruct (Symbol_identifier_as_MiniDecidableType.eq_dec i i0) as [E | ?]; try (right; congruence).
+      inversion E; subst; clear E.
+      destruct (IHa a0); try (right; congruence); subst.
+      left; reflexivity.
+    - intros p a1 IHa2 IHa1 t0.
+      destruct t0; try (right; discriminate).
+      destruct p as [a2 i].
+      destruct p0 as [a2' i'].
+      destruct (Symbol_identifier_as_MiniDecidableType.eq_dec i i') as [E | ?]; try (right; congruence).
+      inversion E; subst; clear E.
+      cbn in *.
+      destruct (IHa1 a); try (right; congruence); subst.
+      destruct (IHa2 a2'); try (right; congruence); subst.
+      left; reflexivity.
+    - intros s l IHl t0.
+      destruct t0; try (right; discriminate).
+      destruct (Sym_t_as_MiniDecidableType.eq_dec s s0) as [E | ?]; try (right; congruence).
+      inversion E; subst; clear E.
+      revert l0.
+      induction IHl as [| [i a] l IHa _ IHl]; intros l0.
+      + destruct l0; try (right; discriminate).
+        left; reflexivity.
+      + destruct l0; try (right; discriminate).
+        destruct p as [i0 a0].
+        destruct (Symbol_identifier_as_MiniDecidableType.eq_dec i i0) as [E | ?]; try (right; congruence).
+        inversion E; subst; clear E.
+        destruct (IHa a0) as [E | ?]; try (right; congruence); subst.
+        destruct (IHl l0) as [E | ?]; try (right; congruence).
+        inversion E; subst; clear E.
+        left; reflexivity.
+    - intros a s i IHa t0.
+      destruct t0; try (right; discriminate).
+      destruct (Symbol_identifier_as_MiniDecidableType.eq_dec i i0) as [E | ?]; try (right; congruence).
+      inversion E; subst; clear E.
+      destruct (Sym_t_as_MiniDecidableType.eq_dec s s0) as [E | ?]; try (right; congruence).
+      inversion E; subst; clear E.
+      destruct (IHa a0); try (right; congruence); subst.
+      left; reflexivity.
+    - intros a1 ct a2 IHa1 IHa2 t0.
+      destruct t0; try (right; discriminate).
+      destruct (SCtypes_as_MiniDecidableType.eq_dec ct t) as [E | ?]; try (right; congruence).
+      inversion E; subst; clear E.
+      destruct (IHa1 a); try (right; congruence); subst.
+      destruct (IHa2 a0); try (right; congruence); subst.
+      left; reflexivity.
+    - intros a1 a2 IHa1 IHa2 t0.
+      destruct t0; try (right; discriminate).
+      destruct (IHa1 a); try (right; congruence); subst.
+      destruct (IHa2 a0); try (right; congruence); subst.
+      left; reflexivity.
+    - intros a IHa t0.
+      destruct t0; try (right; discriminate).
+      destruct (IHa a0); try (right; congruence); subst.
+      left; reflexivity.
+    - intros ct t0.
+      destruct t0; try (right; discriminate).
+      destruct (SCtypes_as_MiniDecidableType.eq_dec ct t) as [E | ?]; try (right; congruence).
+      inversion E; subst; clear E.
+      left; reflexivity.
+    - intros s i t0.
+      destruct t0; try (right; discriminate).
+      destruct (Symbol_identifier_as_MiniDecidableType.eq_dec i i0) as [E | ?]; try (right; congruence).
+      inversion E; subst; clear E.
+      destruct (Sym_t_as_MiniDecidableType.eq_dec s s0) as [E | ?]; try (right; congruence).
+      inversion E; subst; clear E.
+      left; reflexivity.
+    - intros bt t0.
+      destruct t0; try (right; discriminate).
+      destruct (BasetTypes_t_as_MiniDecidableType.eq_dec bt t) as [E | ?]; try (right; congruence).
+      inversion E; subst; clear E.
+      left; reflexivity.
+    - intros a1 a2 IHa1 IHa2 t0.
+      destruct t0; try (right; discriminate).
+      destruct (IHa1 a); try (right; congruence); subst.
+      destruct (IHa2 a0); try (right; congruence); subst.
+      left; reflexivity.
+    - intros a IHa t0.
+      destruct t0; try (right; discriminate).
+      destruct (IHa a0); try (right; congruence); subst.
+      left; reflexivity.
+    - intros a IHa t0.
+      destruct t0; try (right; discriminate).
+      destruct (IHa a0); try (right; congruence); subst.
+      left; reflexivity.
+    - intros a1 a2 a3 IHa1 IHa2 IHa3 t0.
+      destruct t0; try (right; discriminate).
+      destruct (IHa1 a); try (right; congruence); subst.
+      destruct (IHa2 a0); try (right; congruence); subst.
+      destruct (IHa3 a4); try (right; congruence); subst.
+      left; reflexivity.
+    - intros a1 a2 a3 IHa1 IHa2 IHa3 t0.
+      destruct t0; try (right; discriminate).
+      destruct (IHa1 a); try (right; congruence); subst.
+      destruct (IHa2 a0); try (right; congruence); subst.
+      destruct (IHa3 a4); try (right; congruence); subst.
+      left; reflexivity.
+    - intros ct a IHa t0.
+      destruct t0; try (right; discriminate).
+      destruct (SCtypes_as_MiniDecidableType.eq_dec ct t) as [E | ?]; try (right; congruence).
+      inversion E; subst; clear E.
+      destruct (IHa a0); try (right; congruence); subst.
+      left; reflexivity.
+    - intros ct a IHa t0.
+      destruct t0; try (right; discriminate).
+      destruct (SCtypes_as_MiniDecidableType.eq_dec ct t) as [E | ?]; try (right; congruence).
+      inversion E; subst; clear E.
+      destruct (IHa a0); try (right; congruence); subst.
+      left; reflexivity.
+    - intros a1 a2 IHa1 IHa2 t0.
+      destruct t0; try (right; discriminate).
+      destruct (IHa1 a); try (right; congruence); subst.
+      destruct (IHa2 a0); try (right; congruence); subst.
+      left; reflexivity.
+    - intros it a IHa t0.
+      destruct t0; try (right; discriminate).
+      destruct (IntegerType_as_MiniDecidableType.eq_dec it t) as [E | ?]; try (right; congruence).
+      inversion E; subst; clear E.
+      destruct (IHa a0); try (right; congruence); subst.
+      left; reflexivity.
+    - intros bt a IHa t0.
+      destruct t0; try (right; discriminate).
+      destruct (BasetTypes_t_as_MiniDecidableType.eq_dec bt t) as [E | ?]; try (right; congruence).
+      inversion E; subst; clear E.
+      destruct (IHa a0); try (right; congruence); subst.
+      left; reflexivity.
+    - intros a1 a2 a3 IHa1 IHa2 IHa3 t0.
+      destruct t0; try (right; discriminate).
+      destruct (IHa1 a); try (right; congruence); subst.
+      destruct (IHa2 a0); try (right; congruence); subst.
+      destruct (IHa3 a4); try (right; congruence); subst.
+      left; reflexivity.
+    - intros a1 a2 IHa1 IHa2 t0.
+      destruct t0; try (right; discriminate).
+      destruct (IHa1 a); try (right; congruence); subst.
+      destruct (IHa2 a0); try (right; congruence); subst.
+      left; reflexivity.
+    - intros p a IHa t0.
+      destruct t0; try (right; discriminate).
+      destruct p as [s bt].
+      destruct p0 as [s' bt'].
+      destruct (Sym_t_as_MiniDecidableType.eq_dec s s') as [E | ?]; try (right; congruence).
+      inversion E; subst; clear E.
+      destruct (BasetTypes_t_as_MiniDecidableType.eq_dec bt bt') as [E | ?]; try (right; congruence).
+      inversion E; subst; clear E.
+      destruct (IHa a0); try (right; congruence); subst.
+      left; reflexivity.
+    - intros s l IHl t0.
+      destruct t0; try (right; discriminate).
+      destruct (Sym_t_as_MiniDecidableType.eq_dec s s0) as [E | ?]; try (right; congruence).
+      inversion E; subst; clear E.
+      revert l0.
+      induction IHl as [| [t tt] l IHa _ IHl]; intros l0.
+      + destruct l0; try (right; discriminate).
+        left; reflexivity.
+      + destruct l0; try (right; discriminate).
+        destruct (IHa a) as [E | ?]; try (right; congruence).
+        destruct a.
+        inversion E; subst; clear E.
+        destruct (IHl l0) as [E | ?]; try (right; congruence).
+        inversion E; subst; clear E.
+        left; reflexivity.
+    - intros p a IHa2 IHa1 t0.
+      destruct t0; try (right; discriminate).
+      destruct p as [s a2].
+      destruct p0 as [s' a2'].
+      cbn in *.
+      destruct (Sym_t_as_MiniDecidableType.eq_dec s s') as [E | ?]; try (right; congruence).
+      inversion E; subst; clear E.
+      destruct (IHa1 a0); try (right; congruence); subst.
+      destruct (IHa2 a2'); try (right; congruence); subst.
+      left; reflexivity.
+    - intros a1 l IHa IHl t0.
+      destruct t0; try (right; discriminate).
+      destruct (IHa a); try (right; congruence); subst.
+      revert l0.
+      induction IHl as [| [p a2] l IHa2 _ IHl]; intros l0.
+      + destruct l0; try (right; discriminate).
+        left; reflexivity.
+      + destruct l0; try (right; discriminate).
+        destruct p0 as [p' a2'].
+        destruct (Pattern_as_MiniDecidableType.eq_dec p p') as [E | ?]; try (right; congruence).
+        inversion E; subst; clear E.
+        destruct (IHa2 a2'); try (right; congruence); subst.
+        destruct (IHl l0) as [E | ?]; try (right; congruence).
+        inversion E; subst; clear E.
+        left; reflexivity.
+    - intros bt a IHa t0.
+      destruct t0; try (right; discriminate).
+      destruct (BasetTypes_t_as_MiniDecidableType.eq_dec bt t) as [E | ?]; try (right; congruence).
+      inversion E; subst; clear E.
+      destruct (IHa a0); try (right; congruence); subst.
+      left; reflexivity.
+    - intros t tt lc IHt a.
+      destruct a; try (right; discriminate).
+      destruct (Ty_as_MiniDecidableType.eq_dec tt t1); try (right; congruence); subst.
+      destruct (Locations_t_as_MiniDecidableType.eq_dec lc t2) as [E | ?]; try (right; congruence).
+      inversion E; subst; clear E.
+      destruct (IHt t0); try (right; congruence); subst.
+      left; reflexivity.
+  Defined.
+
+  Definition t := term ty.
+  Definition eq := @eq t.
+End Term_as_MiniDecidableType.
+
+Module Annot_as_MiniDecidableType (Ty_as_MiniDecidableType : MiniDecidableType) <: MiniDecidableType.
+  Module Term_as_MiniDecidableType := Term_as_MiniDecidableType Ty_as_MiniDecidableType.
+  Definition ty := Ty_as_MiniDecidableType.t.
+  Definition t := annot ty.
+  Definition eq := @eq t.
+  Lemma eq_dec : forall (x y : t), { eq x y } + { ~ eq x y }.
+  Proof.
+    unfold eq.
+    intros [t1 tt1 lc1] [t2 tt2 lc2].
+    destruct (Term_as_MiniDecidableType.eq_dec t1 t2); try (right; congruence); subst.
+    destruct (Ty_as_MiniDecidableType.eq_dec tt1 tt2); try (right; congruence); subst.
+    destruct (Locations_t_as_MiniDecidableType.eq_dec lc1 lc2) as [E | NE]; try (right; congruence).
+    inversion E; subst; left; reflexivity.
+  Defined.
+End Annot_as_MiniDecidableType.
