coq/Reasoning/ResourceInference.v
@@ -3,136 +3,769 @@ Require Import Coq.ZArith.ZArith.
 Require Import Coq.FSets.FSetInterface.
 
 From Cerberus Require Import IntegerType Ctype.
-From Cn Require Import Prooflog Request Resource Context Sym IndexTerms BaseTypes SCtypes.
+From Cn Require Import Prooflog Request Resource Context Sym IndexTerms BaseTypes SCtypes Global LogicalConstraints.
 
 Import ListNotations.
 
-(* Helper functoin to get a set of resources from the contex *)
 
+(* This is a placeholder for the actual definition of `provable`.
+   The actual definition should be using a proof witness from
+   the SMT solver, which will be checked via SMTCoq plugin.
+ *)
+Inductive provable (g:Global.t): LCSet.t -> LogicalConstraints.t -> Prop :=
+| solvable_SMT: forall lc it, provable g lc it.
+
+(* Helper function to get a set of resources from the contex *)
 Definition ctx_resources_set (l:((list (Resource.t * Z)) * Z)) : ResSet.t
   :=
   Resource.set_from_list (List.map fst (fst l)).
+
+Inductive term_is_struct: Terms.term BaseTypes.t -> Prop :=
+| term_is_struct_intro: forall tag fields,
+  term_is_struct (Terms.Struct _ tag fields).
+
+Lemma term_is_struct_dec: forall t, (term_is_struct t) + (~ term_is_struct t).
+Proof.
+  intros t.
+  destruct t.
+  all: try (left; constructor).
+  all: try (right; intros H; inversion H).
+Qed.
 
 (* Relation between Sctypes.t and BaseTypes.t *)
 Inductive bt_of_sct_rel : SCtypes.t -> BaseTypes.t -> Prop :=
 | bt_of_sct_void : bt_of_sct_rel SCtypes.Void (BaseTypes.Unit unit)
 | bt_of_sct_integer : forall ity,
-    bt_of_sct_rel (SCtypes.Integer ity) 
-      (BaseTypes.Bits _ (if Memory.is_signed_integer_type ity then BaseTypes.Signed else BaseTypes.Unsigned)
-                      (Memory.sizeof_ity ity * 8))
+  bt_of_sct_rel (SCtypes.Integer ity)
+    (BaseTypes.Bits _ (if Memory.is_signed_integer_type ity then BaseTypes.Signed else BaseTypes.Unsigned)
+       (Memory.sizeof_ity ity * 8))
 | bt_of_sct_array : forall sct bt,
-    bt_of_sct_rel sct bt ->
-    bt_of_sct_rel (SCtypes.Array (sct, None)) 
-      (BaseTypes.Map _ 
-        (BaseTypes.Bits _ BaseTypes.Unsigned (Memory.sizeof_ity (IntegerType.Signed Intptr_t) * 8)) 
-        bt)
+  bt_of_sct_rel sct bt ->
+  bt_of_sct_rel (SCtypes.Array (sct, None))
+    (BaseTypes.Map _
+       (BaseTypes.Bits _ BaseTypes.Unsigned (Memory.sizeof_ity (IntegerType.Signed Intptr_t) * 8))
+       bt)
 | bt_of_sct_pointer : forall sct,
-    bt_of_sct_rel (SCtypes.Pointer sct) (BaseTypes.Loc unit tt)
+  bt_of_sct_rel (SCtypes.Pointer sct) (BaseTypes.Loc unit tt)
 | bt_of_sct_struct : forall tag,
-    bt_of_sct_rel (SCtypes.Struct tag) (BaseTypes.Struct _ tag)
+  bt_of_sct_rel (SCtypes.Struct tag) (BaseTypes.Struct _ tag)
 (* TODO function types *).
 
-(* Helper predicate to relate struct piece to resource *)
-Inductive struct_piece_to_resource 
-  (piece: Memory.struct_piece) 
-  (iinit: init) 
-  (ipointer: IndexTerms.t) 
-  (iargs: list IndexTerms.t) 
-  (tag: Sym.t) 
-  (loc: Location.t)
-  : output -> Resource.t -> Prop :=
-| struct_piece_to_resource_intro:
-    forall pid pty field_bt fields field_it struct_loc,
-    Memory.piece_member_or_padding piece = Some (pid, pty) ->
-    let field_pointer := Terms.IT _ (Terms.MemberShift _ ipointer tag pid) (BaseTypes.Loc _ tt) loc in
-    let field_out := Resource.O field_it in
-    (* The field's type maps to its base type *)
-    bt_of_sct_rel pty field_bt ->
-    (* field_out is the IT corresponding to pid in iout's field list *)
-    List.In (pid, field_it) fields 
-    
-    ->
+Definition bool_of_sum {P : Prop} (dec : sumbool P (~ P)) : bool :=
+  match dec with
+  | left _ => true
+  | right _ => false
+  end.
 
-    struct_piece_to_resource piece iinit ipointer iargs tag loc 
+Fixpoint bt_of_sct_fun (sct : SCtypes.t) (bt : BaseTypes.t): bool :=
+  match sct with
+  | SCtypes.Void =>
+    match bt with
+    | BaseTypes.Unit _ => true
+    | _ => false
+    end
+  | SCtypes.Integer ity =>
+      bool_of_sum
+        (BasetTypes_t_as_MiniDecidableType.eq_dec bt
+          (BaseTypes.Bits _ (if Memory.is_signed_integer_type ity then BaseTypes.Signed else BaseTypes.Unsigned)
+                            (Memory.sizeof_ity ity * 8)))
+  | SCtypes.Array (sct, None) =>
+    match bt with
+    | BaseTypes.Map _ bt1 bt2 =>
+      bt_of_sct_fun sct bt2 &&
+      bool_of_sum
+        (BasetTypes_t_as_MiniDecidableType.eq_dec bt1
+          (BaseTypes.Bits _ BaseTypes.Unsigned (Memory.sizeof_ity (IntegerType.Signed Intptr_t) * 8)))
+    | _ => false
+    end
+  | SCtypes.Pointer sct =>
+    match bt with
+    | BaseTypes.Loc _ tt => true
+    | _ => false
+    end
+  | SCtypes.Struct tag1 =>
+    match bt with
+    | BaseTypes.Struct _ tag2 => 
+      if Sym_t_as_MiniDecidableType.eq_dec tag1 tag2
+      then true else false
+    | _ => false
+    end
+  | _ => false
+  end.
+
+Lemma eq_dec_refl_l {A : Type} (x : A) (eq_dec : forall x y : A, {x = y} + {x <> y}) :
+  bool_of_sum (eq_dec x x) = true.
+Proof.
+  destruct (eq_dec x x) as [H | H]; auto.
+Qed.
+
+Lemma eq_dec_refl_r {A : Type} (x y : A) (eq_dec : forall x y : A, {x = y} + {x <> y}) :
+  bool_of_sum (eq_dec x y) = true -> x = y.
+Proof.
+  destruct (eq_dec x y) as [H | H]; auto.
+  intros ?; discriminate.
+Qed.
+
+Lemma bt_of_sct_rel_fun_eq: forall sct bt,
+  bt_of_sct_rel sct bt <-> bt_of_sct_fun sct bt = true.
+Proof.
+  intros sct bt.
+  split; intros H.
+  - induction H; try reflexivity.
+    + unfold bt_of_sct_fun.
+      apply eq_dec_refl_l.
+    + simpl.
+      rewrite IHbt_of_sct_rel.
+      reflexivity.
+    + simpl.
+      apply eq_dec_refl_l.
+  - revert bt H.
+    apply SCtypes.ctype_ind_set with (P := fun sct => forall bt : BaseTypes.t, bt_of_sct_fun sct bt = true -> bt_of_sct_rel sct bt).
+    + intros bt H.
+      destruct bt; try discriminate.
+      constructor.
+    + intros i bt H.
+      destruct bt; try discriminate.
+      unfold bt_of_sct_fun in H.
+      destruct BasetTypes_t_as_MiniDecidableType.eq_dec as [E | ?]; try discriminate.
+      rewrite E.
+      constructor.
+    + intros [sct' o] IH bt H.
+      destruct o; try discriminate.
+      destruct bt; try discriminate.
+      simpl in IH, H.
+      destruct (bt_of_sct_fun sct' bt2) eqn:H'; try discriminate.
+      destruct BasetTypes_t_as_MiniDecidableType.eq_dec as [E | ?]; try discriminate.
+      clear H.
+      rewrite E.
+      constructor.
+      apply IH, H'.
+    + intros sct' IH bt H.
+      destruct bt; try discriminate.
+      destruct u.
+      constructor.
+    + intros s bt H.
+      destruct bt; try discriminate.
+      simpl in H.
+      destruct Sym_t_as_MiniDecidableType.eq_dec as [E | ?]; try discriminate.
+      rewrite E.
+      constructor.
+    + intros ? ? ? ? H.
+      inversion H.
+Qed.
+
+Lemma bt_of_sct_rel_functional : forall sct bt1 bt2,
+  bt_of_sct_rel sct bt1 ->
+  bt_of_sct_rel sct bt2 ->
+  bt1 = bt2.
+Proof.
+  intros sct bt1 bt2 H1 H2.
+  revert bt2 H2.
+  induction H1; intros bt2 H2.
+  all: inversion H2; subst; clear H2.
+  - reflexivity.
+  - reflexivity.
+  - rewrite IHbt_of_sct_rel with (bt2 := bt0).
+    + reflexivity.
+    + assumption.
+  - reflexivity.
+  - reflexivity.
+Qed.
+
+(* Defines when a term represents a cast of another term to a specific type *)
+Inductive cast_ (loc: Locations.t) : BaseTypes.t -> IndexTerms.t -> IndexTerms.t -> Prop :=
+| cast_same: forall bt t' l',
+  cast_ loc bt (Terms.IT _ t' bt l') (Terms.IT _ t' bt l')
+| cast_diff: forall bt t' bt' l',
+  bt <> bt' ->
+  cast_ loc bt (Terms.IT _ t' bt l') (Terms.IT _ (Terms.Cast _ bt (Terms.IT _ t' bt' l')) bt loc).
+
+(* Defines when a term represents the allocation id of another term *)
+Inductive allocId_ (loc: Locations.t) : IndexTerms.t -> IndexTerms.t -> Prop :=
+| allocId_intro: forall t' bt' l' result,
+  cast_ loc (BaseTypes.Alloc_id _) (Terms.IT _ t' bt' l') result ->
+  allocId_ loc (Terms.IT _ t' bt' l') result.
+
+(* Defines when a term represents the address of another term *)
+Inductive addr_ (loc: Locations.t) : IndexTerms.t -> IndexTerms.t -> Prop :=
+| addr_intro: forall pt t' bt' l' result,
+  bt_of_sct_rel (SCtypes.Integer (IntegerType.Signed Intptr_t)) pt ->
+  cast_ loc pt (Terms.IT _ t' bt' l') result ->
+  addr_ loc (Terms.IT _ t' bt' l') result.
+
+Definition fields_list_functional (fields : list (Symbol.identifier * IndexTerms.t)) : Prop :=
+  forall id field1 field2,
+  List.In (id, field1) fields ->
+  List.In (id, field2) fields ->
+  field1 = field2.
+
+Lemma fields_list_nodup_is_functional : forall fields,
+  NoDup (List.map fst fields) ->
+  fields_list_functional fields.
+Proof.
+  intros fields H id field1 field2 Hfield1 Hfield2.
+  assert (id_def : Symbol.identifier) by (repeat constructor).
+  assert (term_def : IndexTerms.t) by (repeat constructor).
+  apply In_nth with (d := (id_def, term_def)) in Hfield1.
+  apply In_nth with (d := (id_def, term_def)) in Hfield2.
+  destruct Hfield1 as [n1 [Hn1 Hfield1]].
+  destruct Hfield2 as [n2 [Hn2 Hfield2]].
+  apply NoDup_nth with (i := n1) (j := n2) (d := id_def) in H.
+  - rewrite H in Hfield1.
+    rewrite Hfield1 in Hfield2.
+    inversion_clear Hfield2.
+    reflexivity.
+  - rewrite length_map.
+    apply Hn1.
+  - rewrite length_map.
+    apply Hn2.
+  - change id_def with (fst (id_def, term_def)).
+    rewrite 2 map_nth.
+    rewrite Hfield1, Hfield2.
+    cbn.
+    reflexivity.
+Qed.
+
+Lemma NoDup_dec (A : Type)
+  (dec: forall (x y : A), {x = y} + {x <> y})
+  (l : list A): { NoDup l } + { ~ NoDup l }.
+Proof.
+  induction l as [|a l IH].
+  - left; now constructor.
+  - destruct (In_dec dec a l).
+    + right.
+      inversion_clear 1.
+      tauto.
+    + destruct IH.
+      * left.
+        now constructor.
+      * right.
+        inversion_clear 1.
+        tauto.
+Defined.
+
+Lemma NoDup_dec_true : forall A (dec : forall x y : A, {x = y} + {x <> y}) (l : list A),
+  NoDup l <-> bool_of_sum (NoDup_dec _ dec l) = true.
+Proof.
+  intros A dec l.
+  split; intros H.
+  - destruct NoDup_dec; auto.
+  - destruct NoDup_dec; auto.
+    inversion H.
+Qed.
+
+Lemma NoDup_dec_false : forall A (dec : forall x y : A, {x = y} + {x <> y}) (l : list A),
+  ~ NoDup l <-> bool_of_sum (NoDup_dec _ dec l) = false.
+Proof.
+  intros A dec l.
+  split; intros H.
+  - destruct NoDup_dec; auto.
+    exfalso; tauto.
+  - destruct NoDup_dec; auto.
+    inversion H.
+Qed.
+
+(* Helper predicate to relate struct piece to resource *)
+Inductive struct_piece_to_resource
+  (piece: Memory.struct_piece)
+  (iinit: init) (ipointer: IndexTerms.t) (iargs: list IndexTerms.t) (* lhs predicate*)
+  (tag: Sym.t)
+  : output -> Resource.t -> Prop :=
+| struct_piece_to_resource_struct:
+  forall pid pty fields field_it struct_loc,
+  Memory.piece_member_or_padding piece = Some (pid, pty) ->
+  let field_pointer := Terms.IT _ (Terms.MemberShift _ ipointer tag pid) (BaseTypes.Loc _ tt) struct_loc in
+  NoDup (List.map fst fields) ->
+  (* field_out is the IT corresponding to pid in iout's field list *)
+  List.In (pid, field_it) fields
+
+  ->
+
+    struct_piece_to_resource piece iinit ipointer iargs tag
       (Resource.O (Terms.IT _ (Terms.Struct _ tag fields) (BaseTypes.Struct _ tag) struct_loc))
       (Request.P {| Predicate.name := Request.Owned pty iinit;
-                    Predicate.pointer := field_pointer; 
+                   Predicate.pointer := field_pointer;
+                   Predicate.iargs := iargs |},
+       (Resource.O field_it))
+
+| struct_piece_to_resource_opaque:
+  forall pid pty field_bt struct_loc struct_term,
+  Memory.piece_member_or_padding piece = Some (pid, pty) ->
+  let field_pointer := Terms.IT _ (Terms.MemberShift _ ipointer tag pid) (BaseTypes.Loc _ tt) struct_loc in
+  (* The field's type maps to its base type *)
+  bt_of_sct_rel pty field_bt ->
+  let struct_type := (BaseTypes.Struct _ tag) in
+  ~ term_is_struct struct_term
+
+  ->
+
+    struct_piece_to_resource piece iinit ipointer iargs tag
+      (Resource.O (Terms.IT _ struct_term struct_type struct_loc))
+      (Request.P {| Predicate.name := Request.Owned pty iinit;
+                    Predicate.pointer := field_pointer;
                     Predicate.iargs := iargs |},
-       field_out).
+       (Resource.O
+         (Terms.IT _ 
+           (Terms.StructMember _
+             (Terms.IT _ struct_term struct_type struct_loc)
+             pid)
+           field_bt
+           struct_loc))).
 
-Inductive resource_unfold (globals:Global.t): Resource.t -> ResSet.t -> Prop :=
-(* non-struct "Owned" resources unfold to themselves *)
-| resource_unfold_nonstruct:
-    forall ipointer iargs iout iinit ity,
-    not (SCtypes.is_struct ity) ->
+Definition struct_piece_to_resource_fun
+  (piece: Memory.struct_piece)
+  (iinit: init) (ipointer: IndexTerms.t) (iargs: list IndexTerms.t) (* lhs predicate*)
+  (tag: Sym.t)
+  (out : output) (res : Resource.t) : bool :=
+  match res with
+  | (Request.P req, Resource.O field_it) =>
+    match out with
+    | Resource.O (Terms.IT _ struct_term struct_type struct_loc) =>
+      match Memory.piece_member_or_padding piece with
+      | Some (pid, pty) =>
+        let field_pointer := Terms.IT _ (Terms.MemberShift _ ipointer tag pid) (BaseTypes.Loc _ tt) struct_loc in
+        bool_of_sum (BasetTypes_t_as_MiniDecidableType.eq_dec struct_type (BaseTypes.Struct _ tag)) &&
+        bool_of_sum (Predicate_as_MiniDecidableType.eq_dec req
+          {| Predicate.name := Request.Owned pty iinit;
+             Predicate.pointer := field_pointer;
+             Predicate.iargs := iargs |}) &&
+        match struct_term with
+        | Terms.Struct _ tag' fields =>
+          bool_of_sum (NoDup_dec _ Symbol_identifier_as_MiniDecidableType.eq_dec (List.map fst fields)) &&
+          List.existsb (fun '(pid', field_it') =>
+                          bool_of_sum (Symbol_identifier_as_MiniDecidableType.eq_dec pid pid') &&
+                          bool_of_sum (IndexTerm_as_MiniDecidableType.eq_dec field_it field_it'))
+                        fields &&
+          bool_of_sum (Sym_t_as_MiniDecidableType.eq_dec tag tag')
+        | _ =>
+          match field_it with
+          | Terms.IT _  output_term field_bt loc =>
+            bt_of_sct_fun pty field_bt &&
+            bool_of_sum (IndexTerm_as_MiniDecidableType.eq_dec
+              (Terms.IT _ output_term field_bt loc)
+              (Terms.IT _ (Terms.StructMember _ (Terms.IT _ struct_term struct_type struct_loc) pid) field_bt struct_loc))
+          end
+        end
+      | _ => false
+      end
+    end
+  | _ => false
+  end.
 
-    resource_unfold globals
-      (Request.P 
-        {| 
-          Predicate.name := Request.Owned ity iinit; 
-          Predicate.pointer := ipointer; 
-          Predicate.iargs := iargs 
-        |}, 
-        iout) 
-      (ResSet.singleton 
-        (Request.P 
-        {| 
-          Predicate.name := Request.Owned ity iinit; 
-          Predicate.pointer := ipointer; 
-          Predicate.iargs := iargs 
-        |}, 
-        iout)         
-      ) 
+Lemma struct_piece_to_resource_functional:
+  forall piece iinit ipointer iargs tag out res1 res2,
+  struct_piece_to_resource piece iinit ipointer iargs tag out res1 ->
+  struct_piece_to_resource piece iinit ipointer iargs tag out res2 ->
+  res1 = res2.
+Proof.
+  intros piece iinit ipointer iargs tag out res1 res2 H1 H2.
+  inversion H1; inversion H2; subst; clear H1 H2.
+  - inversion H9; subst; clear H9.
+    rewrite H in H6; inversion H6; subst; clear H6.
+    unfold field_pointer, field_pointer0.
+    repeat (f_equal; auto).
+    apply fields_list_nodup_is_functional in H7.
+    eapply H7; eauto.
+  - inversion H9; subst; clear H9.
+    exfalso.
+    apply H8.
+    constructor.
+  - inversion H9; subst; clear H9.
+    exfalso.
+    apply H3.
+    constructor.
+  - inversion H9; subst; clear H9.
+    unfold field_pointer, field_pointer0.
+    rewrite H in H6; inversion H6; subst; clear H6.
+    repeat (f_equal; auto).
+    eapply bt_of_sct_rel_functional; eauto.
+Qed.
 
-| resource_unfold_struct:
-  forall out_res ipointer iargs iout iinit isym sdecl loc,
+Lemma struct_piece_to_resource_fun_eq:
+  forall piece iinit ipointer iargs tag out res,
+  struct_piece_to_resource piece iinit ipointer iargs tag out res <->
+  struct_piece_to_resource_fun piece iinit ipointer iargs tag out res = true.
+Proof.
+  intros piece iinit ipointer iargs tag out res.
+  split.
+  - intros H.
+    unfold struct_piece_to_resource_fun.
+    destruct res as [req [field_it]].
+    destruct req as [P | Q]; [| inversion H].
+    destruct P as [name pointer args].
+    destruct out as [[]].
+    inversion H; subst.
+    + unfold field_pointer.
+      rewrite H4.
+      epose proof (existsb_exists _ _) as He.
+      destruct He as [_ He].
+      rewrite He; revgoals.
+      { exists (pid, field_it).
+        split; auto.
+        apply andb_true_intro; split; apply eq_dec_refl_l. }
+      repeat (apply andb_true_intro; split); auto.
+      all: try apply eq_dec_refl_l.
+      apply NoDup_dec_true, H8.
+    + unfold field_pointer.
+      rewrite H4.
+      apply bt_of_sct_rel_fun_eq in H8.
+      rewrite H8.
+      unfold struct_type.
+      rewrite eq_dec_refl_l with (eq_dec := BasetTypes_t_as_MiniDecidableType.eq_dec).
+      rewrite eq_dec_refl_l with (eq_dec := Predicate_as_MiniDecidableType.eq_dec).
+      rewrite eq_dec_refl_l with (eq_dec := IndexTerm_as_MiniDecidableType.eq_dec).
+      destruct t; auto.
+      exfalso.
+      apply H9.
+      constructor.
+  - intros H.
+    unfold struct_piece_to_resource_fun in H.
+    destruct res as [req [field_it]].
+    destruct req as [P | Q]; try discriminate.
+    destruct P as [name pointer args].
+    destruct pointer.
+    destruct out as [[]].
+    destruct Memory.piece_member_or_padding as [[pid pty]|] eqn:E; try discriminate.
+    apply andb_prop in H; destruct H as [H1 H2].
+    apply andb_prop in H1; destruct H1 as [H1 H3].
+    apply eq_dec_refl_r in H3.
+    inversion H3; subst; clear H3.
+    destruct (term_is_struct_dec t2) as [Ht | Ht].
+    + inversion Ht; subst; clear Ht.
+      apply andb_prop in H2; destruct H2 as [H2 H4].
+      apply andb_prop in H2; destruct H2 as [H2 H5].
+      apply NoDup_dec_true in H2.
+      epose proof (existsb_exists _ _) as He.
+      destruct He as [He _].
+      apply He in H5; clear He.
+      destruct H5 as [[pid' field_it'] [H0 H5]].
+      apply andb_prop in H5; destruct H5 as [H5 H6].
+      apply eq_dec_refl_r in H1, H4, H5, H6; subst.
+      apply struct_piece_to_resource_struct.
+      all: assumption.
+    + destruct t2; try (exfalso; apply Ht; constructor).
+      all: destruct field_it; try discriminate.
+      all: apply andb_prop in H2; destruct H2 as [H2 H4].
+      all: apply eq_dec_refl_r in H1, H4; subst.
+      all: inversion H4; subst; clear H4.
+      all: apply bt_of_sct_rel_fun_eq in H2.
+      all: apply struct_piece_to_resource_opaque.
+      all: assumption.
+Qed.
 
+(* computable version of subsumed predicate*)
+Definition subsumed_fun (p1 p2 : Request.name) : bool :=
+  orb
+    (bool_of_sum (Name_as_MiniDecidableType.eq_dec p1 p2))
+    (match p1, p2 with
+     | Request.Owned ct Uninit, Request.Owned ct' Init
+         => bool_of_sum (SCtypes_as_MiniDecidableType.eq_dec ct ct')
+     | _, _ => false
+     end).
+
+(* Equivalence between subsumed and subsumed_fun *)     
+Lemma subsumed_fun_eq:
+  forall p1 p2,
+  subsumed p1 p2 <-> subsumed_fun p1 p2 = true.
+Proof.
+  intros p1 p2.
+  split.
+  - intros H.
+    unfold subsumed_fun.
+    apply orb_true_intro.
+    inversion H; subst.
+    + left.
+      apply eq_dec_refl_l.
+    + right.
+      apply eq_dec_refl_l.
+  - intros H.
+    unfold subsumed_fun in H.
+    apply orb_prop in H; destruct H as [H | H].
+    + apply Subsumed_equal.
+      eapply eq_dec_refl_r, H.
+    + destruct p1; try discriminate.
+      destruct i; try discriminate.
+      destruct p2; try discriminate.
+      destruct i; try discriminate.
+      apply Subsumed_owned.
+      eapply eq_dec_refl_r, H.
+Qed.
+
+Inductive unfold_one (globals:Global.t): Resource.t -> ResSet.t -> Prop :=
+| unfold_one_struct:
+  forall out_res ipointer iargs iout iinit iinit' isym sdecl,
+
+  let iname := Request.Owned (SCtypes.Struct isym) iinit in
+  let iname' := Request.Owned (SCtypes.Struct isym) iinit' in
+
+  subsumed iname iname' ->
+  
   (* lookup struct declaration in global environment *)
   SymMap.MapsTo isym sdecl globals.(Global.struct_decls) ->
 
   (* Resources are related to struct pieces *)
-  (forall r, 
-    ResSet.In r out_res <->
-      exists piece, List.In piece sdecl /\
-        struct_piece_to_resource piece iinit ipointer iargs isym loc iout r) 
-  
+  (forall r,
+     ResSet.In r out_res <->
+       exists piece, List.In piece sdecl /\
+                struct_piece_to_resource piece iinit' ipointer iargs isym iout r)
+
   ->
 
-  resource_unfold globals
-    (Request.P 
-      {| 
-        Predicate.name := Request.Owned (SCtypes.Struct isym) iinit; 
-        Predicate.pointer := ipointer; 
-        Predicate.iargs := iargs 
-      |}, 
-      iout) 
-    out_res.
-  
+    unfold_one globals
+      (Request.P
+         {|
+           Predicate.name := iname;
+           Predicate.pointer := ipointer;
+           Predicate.iargs := iargs
+         |},
+         iout)
+      out_res.
+
+(* Computable version of unfold_one predicate *) 
+Definition unfold_one_fun (globals:Global.t) (r : Resource.t) (out_res: list Resource.t) : bool :=
+  match r with
+  | (Request.P {|
+        Predicate.name := Request.Owned (SCtypes.Struct isym) iinit;
+        Predicate.pointer := ipointer;
+        Predicate.iargs := iargs
+      |} , iout) =>
+        match SymMap.find isym globals.(Global.struct_decls) with
+        | Some sdecl =>
+          (List.length sdecl =? List.length out_res) &&
+          List.forallb
+            (fun '(piece, r) => struct_piece_to_resource_fun piece iinit ipointer iargs isym iout r)
+            (List.combine sdecl out_res)
+        | None => false
+        end
+  | _ => false
+  end.
+
+(* Equivalence between unfold_one and unfold_one_fun *)
+Lemma unfold_one_fun_eq:
+  forall globals r out_res,
+  unfold_one_fun globals r out_res = true ->
+  unfold_one globals r (Resource.set_from_list out_res).
+Proof.
+  intros globals r out_res H.
+  unfold unfold_one_fun in H.
+  destruct r as [req out].
+  destruct req as [P | Q]; try discriminate; subst.
+  destruct P as [name pointer args].
+  destruct name; try discriminate.
+  destruct t; try discriminate.
+  destruct SymMap.find eqn:Hf; try discriminate.
+  apply andb_prop in H; destruct H as [HlEQ H].
+  apply Nat.eqb_eq in HlEQ.
+  apply SymMap.find_2 in Hf.
+  assert (piece_def : Memory.struct_piece) by (repeat constructor).
+  assert (res_def : Resource.t) by (repeat constructor).
+  eapply unfold_one_struct with (iinit' := i).
+  { apply Subsumed_equal.
+    reflexivity. }
+  { apply Hf. }
+  intros r; split.
+  - intros Hr.
+    apply ResSet_In_List_In_eq in Hr.
+    eapply In_nth with (d := res_def) in Hr as [n [Hl_out_res Hnth]].
+    eapply forallb_forall in H; revgoals.
+    { apply nth_In with (n := n).
+      rewrite length_combine, HlEQ, Nat.min_id.
+      apply Hl_out_res. }
+    rewrite combine_nth with (x := piece_def) (y := res_def) in H by (apply HlEQ).
+    rewrite <- Hnth.
+    exists (nth n s0 piece_def); split.
+    + apply nth_In.
+      rewrite HlEQ.
+      apply Hl_out_res.
+    + apply struct_piece_to_resource_fun_eq, H.
+  - intros [piece [Hp H1]].
+    apply ResSet_In_List_In_eq.
+    eapply In_nth with (d := piece_def) in Hp as [n [Hl_s0 Hnth]].
+    eapply forallb_forall in H; revgoals.
+    { apply nth_In with (n := n).
+      rewrite length_combine, <- HlEQ, Nat.min_id.
+      apply Hl_s0. }
+    rewrite combine_nth with (x := piece_def) (y := res_def) in H by (apply HlEQ).
+    rewrite Hnth in H.
+    apply struct_piece_to_resource_fun_eq in H.
+    erewrite struct_piece_to_resource_functional with (res1 := r) (res2 := nth n out_res res_def).
+    + apply nth_In.
+      rewrite <- HlEQ.
+      apply Hl_s0.
+    + apply H1.
+    + apply H.
+Qed.
+
+Inductive unfold_all (globals:Global.t): ResSet.t -> ResSet.t -> Prop :=
+| unfold_all_step:
+    forall input input' output r unfolded_r,
+    (* Find a resource that can be unfolded *)
+    ResSet.In r input ->
+    unfold_one globals r unfolded_r ->
+    (* Continue unfolding with the resource replaced by its unfolded components *)
+    ResSet.Equal input' (ResSet.union (ResSet.remove r input) unfolded_r) ->
+    unfold_all globals input' output ->
+    (* This is the result of unfolding the input *)
+    unfold_all globals input output
+| unfold_all_fixpoint:
+    forall input output,
+    (* A fixpoint is reached when no resource can be unfolded further *)
+    ~ ResSet.Exists
+        (fun r => exists unfolded_r, unfold_one globals r unfolded_r)
+        input ->
+    ResSet.Equal input output ->
+    unfold_all globals input output.
+
+(* A version of `unfold_all`, using hints *)
+Inductive unfold_all_explicit (globals:Global.t):
+  list (Resource.t * unpack_result) -> ResSet.t -> ResSet.t -> Prop :=
+| unfold_all_explicit_step:
+    forall input input' output r unfolded_r_list unfold_changed,
+    let unfolded_r_set := Resource.set_from_list unfolded_r_list in
+    (* Find a resource that can be unfolded *)
+    ResSet.In r input ->
+    unfold_one globals r unfolded_r_set ->
+    (* Continue unfolding with the resource replaced by its unfolded components *)
+    ResSet.Equal input' (ResSet.union (ResSet.remove r input) unfolded_r_set) ->
+    unfold_all_explicit globals unfold_changed input' output ->
+    (* This is the result of unfolding the input *)
+    unfold_all_explicit globals ((r, UnpackRES unfolded_r_list) :: unfold_changed) input output
+| unfold_all_explicit_fixpoint:
+    forall input output,
+    (* A fixpoint is reached when no resource can be unfolded further *)
+    ~ ResSet.Exists
+        (fun r => exists unfolded_r, unfold_one globals r unfolded_r)
+        input ->
+    ResSet.Equal input output ->
+    unfold_all_explicit globals [] input output.
+
+(* Proof that unfold_all_explicit is equivalent to unfold_all *)    
+Lemma unfold_all_explicit_eq:
+  forall globals input output unfold_changed,
+  unfold_all_explicit globals unfold_changed input output ->
+  unfold_all globals input output.
+Proof.
+  intros globals input output unfold_changed H.
+  induction H.
+  - eapply unfold_all_step; eassumption.
+  - eapply unfold_all_fixpoint; eassumption.
+Qed.
+
+Definition resource_is_struct (r : Resource.t): bool :=
+  match r with
+  | (Request.P {| Predicate.name := Request.Owned (SCtypes.Struct _) _;
+                  Predicate.pointer := _;
+                  Predicate.iargs := _ |}, _) =>
+    true
+  | _ => false
+  end.
+
+(* Computable version of unfold_all_explicit predicate *)
+Fixpoint unfold_all_explicit_fun
+  (globals:Global.t)
+  (unfold_changed : list (Resource.t * unpack_result))
+  (input output: list Resource.t): bool :=
+  match unfold_changed with
+  | ((r, UnpackRES unfolded_r_list) :: unfold_changed) =>
+    let input' := List.app (List.remove Resource_as_DecidableType.eq_dec r input) unfolded_r_list in
+    List.existsb (fun r' => bool_of_sum (Resource_as_DecidableType.eq_dec r r')) input &&
+    unfold_one_fun globals r unfolded_r_list &&
+    unfold_all_explicit_fun globals unfold_changed input' output
+  | [] =>
+    negb (List.existsb resource_is_struct input) && (* this should be updated later to support arrays *)
+    ResSet.equal (Resource.set_from_list input) (Resource.set_from_list output)
+  | _ => false
+  end.
+
+(* Equivalence between unfold_all_explicit and unfold_all_explicit_fun *)
+Lemma unfold_all_explicit_fun_eq:
+  forall globals input output unfold_changed,
+  unfold_all_explicit_fun globals unfold_changed input output = true ->
+  unfold_all_explicit globals unfold_changed (Resource.set_from_list input) (Resource.set_from_list output).
+Proof.
+  intros globals input output unfold_changed.
+  revert input output.
+  induction unfold_changed; intros input output H.
+  - simpl in H.
+    apply andb_prop in H; destruct H as [H1 H2].
+    eapply unfold_all_explicit_fixpoint.
+    + intros H.
+      enough (true = false) by discriminate.
+      rewrite <- H1.
+      apply negb_false_iff.
+      destruct H as [r [Hr [unfolded_r H]]].
+      apply existsb_exists.
+      exists r; split.
+      * apply ResSet_In_List_In_eq, Hr.
+      * destruct r; try inversion H.
+        reflexivity.
+    + apply ResSetDecide.F.equal_iff, H2.
+  - destruct a as [r unpack_r].
+    destruct unpack_r as [? | unfolded_r]; try discriminate.
+    cbn in H.
+    apply andb_prop in H; destruct H as [H1 H2].
+    apply andb_prop in H1; destruct H1 as [H1 H3].
+    apply existsb_exists in H1.
+    destruct H1 as [r' [Hr' H1]].
+    apply eq_dec_refl_r in H1; subst.
+    eapply unfold_all_explicit_step
+    with (input' := Resource.set_from_list (remove ResSetDecide.F.eq_dec r' input ++ unfolded_r)).
+    + apply ResSet_In_List_In_eq, Hr'.
+    + apply unfold_one_fun_eq, H3.
+    + clear.
+      unfold ResSet.Equal.
+      intros r; split; intros H.
+      * apply ResSet_In_List_In_eq in H.
+        apply in_app_iff in H.
+        apply ResSetDecide.F.union_iff.
+        destruct H as [H | H].
+        -- left.
+           apply in_remove in H.
+           destruct H as [H1 H2].
+           apply ResSetDecide.F.remove_iff.
+           split.
+           ++ apply ResSet_In_List_In_eq, H1.
+           ++ apply not_eq_sym, H2.
+        -- right.
+           apply ResSet_In_List_In_eq, H.
+      * apply ResSet_In_List_In_eq.
+        apply in_app_iff.
+        apply ResSetDecide.F.union_iff in H.
+        destruct H as [H | H].
+        -- left.
+           apply ResSetDecide.F.remove_iff in H.
+           destruct H as [H1 H2].
+           apply in_in_remove.
+           ++ apply not_eq_sym, H2.
+           ++ apply ResSet_In_List_In_eq, H1.
+        -- right.
+           apply ResSet_In_List_In_eq, H.
+    + apply IHunfold_changed, H2.
+Qed.
+
+Definition unfold_step_flatten (l : list unfold_step): unfold_changed :=
+  List.concat (List.map fst l).
+
 (** Inductive predicate which defines correctness of resource unfolding step *)
 Inductive unfold_step : Context.t -> Context.t -> Prop :=
 | simple_unfold_step:
-    forall 
+  forall
     icomputational ilogical iresources iconstraints iglobal
     ocomputational ological oresources oconstraints oglobal,
-    
+
   (* The following parts of context are not changed *)
-    icomputational = ocomputational ->
-    iglobal = oglobal ->
-    ilogical = ological ->
-    iconstraints = oconstraints ->
+  icomputational = ocomputational ->
+  iglobal = oglobal ->
+  ilogical = ological ->
+  iconstraints = oconstraints ->
 
-    let in_res := ctx_resources_set iresources in
-    let out_res := ctx_resources_set oresources in
+  let in_res := ctx_resources_set iresources in
+  let out_res := ctx_resources_set oresources in
 
-    (* The `out_res` is union of `resource_unfold` of all resources in `in_res` *)
-    (forall r', ResSet.In r' out_res <-> 
-      exists r, ResSet.In r in_res /\ exists s, 
-      resource_unfold iglobal r s /\ ResSet.In r' s
-    ) 
-    
-    ->
+  (* The `out_res` is union of `unfold_one` of all resources in `in_res` *)
+  unfold_all iglobal in_res out_res ->
 
-    unfold_step
+  unfold_step
     (* input context *)
     {|
       Context.computational := icomputational;
@@ -150,122 +783,48 @@ Inductive unfold_step : Context.t -> Context.t -> Prop :=
       Context.constraints := oconstraints;
       Context.global := oglobal
     |}.
-  
+
+(* Helper definition, used in [log_entry_valid] *)
+Local Definition ptr_alloc_id_eq (g: Global.t) (c: LCSet.t) (p p': IndexTerms.t) :=
+  exists loc alloc_id_eq alloc alloc',
+    allocId_ loc p alloc /\
+    allocId_ loc p' alloc' /\
+    IndexTerms.eq_ loc alloc alloc' alloc_id_eq /\
+    provable g c (LogicalConstraints.T alloc_id_eq).
+
+(* Helper definition, used in [log_entry_valid] *)
+Local Definition ptr_addr_and_args_eq (g: Global.t) (c: LCSet.t) (p p': IndexTerms.t) (a a': list IndexTerms.t) :=
+  exists pointer_eq loc,
+    IndexTerms.eq_ loc p p' pointer_eq /\
+    provable g c (LogicalConstraints.T pointer_eq) /\
+    (* arguments match *)
+    (exists addr_iargs_match addr addr',
+        addr_ loc p addr /\
+        addr_ loc p' addr' /\
+        IndexTerms.eq_ loc addr addr' pointer_eq /\
+        IndexTerms.eq_and_list_rel Location.Loc_unknown a a' addr_iargs_match /\
+        provable g c
+          (* we add pointer address equality to the constraint as it might be needed for proving the argument equality *)
+          (LogicalConstraints.T (IndexTerms.and2_ Location.Loc_unknown pointer_eq addr_iargs_match))
+    ).
 
 (** Inductive predicate which defines correctess of log inference step *)
 Inductive log_entry_valid : log_entry -> Prop :=
 | unfold_resources_step:
-    forall loc c c',
-    unfold_step c c' ->
-    log_entry_valid (ResourceInferenceStep c (UnfoldResources loc) c')
+  forall loc c c' steps,
+  unfold_step c c' ->
+  log_entry_valid (UnfoldResources c loc steps c')
 
-(* simple case: non-recursive request, no packing *)
-| simple_resource_inference_step:
-  forall iname  ipointer  iargs
-    oname  opointer  oargs
-    err out lines oloc
-    icomputational ilogical iresources iconstraints iglobal
-    ocomputational ological oresources oconstraints oglobal,
-
-  (* The following parts of context are not changed *)
-  icomputational = ocomputational ->
-  iglobal = oglobal ->
-  ilogical = ological ->
-  iconstraints = oconstraints ->
-
-  let in_res := ctx_resources_set iresources in
-  let out_res := ctx_resources_set oresources in
-
-  (* alt. definition sketch:
-  let res_diff := Resource.ResSet.diff in_res out_res in
-  Resource.ResSet.cardinal res_diff = 1 /\
-  ...
-   *)
-
-  (* [out_res] is a subset of [in_res] with exactly one element [used] removed. *)
-  (exists (upred: Request.Predicate.t),
-      ResSet.Equal (Resource.ResSet.add (P upred, out) out_res) in_res /\
-      Request.subsumed iname upred.(Request.Predicate.name)
-  ) 
-  
-  (* TODO:
-  /\ iname=oname  
-  /\ ipointer=opointer
-  /\ iargs=oargs
-  *)
-  ->
-
-    log_entry_valid
-      (ResourceInferenceStep
-         (* input context *)
-         {|
-           Context.computational := icomputational;
-           Context.logical := ilogical;
-           Context.resources := iresources;
-           Context.constraints := iconstraints;
-           Context.global := iglobal
-         |}
-
-         (* request type *)
-         (PredicateRequest
-            err (* unused *)
-            (* input predicate *)
-            {| Predicate.name:=iname; Predicate.pointer:=ipointer; Predicate.iargs:=iargs |}
-            oloc (* unused *)
-            ((
-                (* output predicate *)
-                {| Predicate.name:=oname; Predicate.pointer:=opointer; Predicate.iargs:=oargs |},
-                  out
-              ), lines (* unused *)
-         ))
-
-         (* output context *)
-         {|
-           Context.computational := ocomputational;
-           Context.logical := ological;
-           Context.resources := oresources;
-           Context.constraints := oconstraints;
-           Context.global := oglobal
-         |}
-      )
-
- (* struct case: struct resource is removed from input context *)
-| struct_resource_inference_step:
-  forall isym iinit ipointer iargs
+| array_resource_inference_step:
+  forall ity isize iinit ipointer iargs
     oname opointer oargs
-    err out lines oloc
+    err out
     icomputational ilogical iresources iconstraints iglobal
-    ocomputational ological oresources oconstraints oglobal,
-
-  (* The following parts of context are not changed *)
-  icomputational = ocomputational ->
-  iglobal = oglobal ->
-  ilogical = ological ->
-  iconstraints = oconstraints ->
-
-  let in_res := ctx_resources_set iresources in
-  let out_res := ctx_resources_set oresources in
-
-  (* Find the struct resource and its fields *)
-  (exists (field_res: ResSet.t),
-      (* The struct unfolds to field resources *)
-      resource_unfold iglobal 
-        (Request.P {| Predicate.name := Request.Owned (SCtypes.Struct isym) iinit;
-                      Predicate.pointer := ipointer;
-                      Predicate.iargs := iargs |}, out)
-        field_res /\
-      (* Output context is input context minus all field resources *)
-      ResSet.Equal out_res (ResSet.diff in_res field_res)
-  ) ->
-
-  (* TODO:
-  /\ iname=oname  
-  /\ ipointer=opointer
-  /\ iargs=oargs
-  *)
+    ocomputational ological oresources oconstraints oglobal
+    steps,
 
   log_entry_valid
-    (ResourceInferenceStep
+    (PredicateRequest
       (* input context *)
       {|
         Context.computational := icomputational;
@@ -274,23 +833,17 @@ Inductive log_entry_valid : log_entry -> Prop :=
         Context.constraints := iconstraints;
         Context.global := iglobal
       |}
-
-      (* request type *)
-      (PredicateRequest
-        err (* unused *)
-        (* input predicate *)
-        {| Predicate.name := Request.Owned (SCtypes.Struct isym) iinit;
-           Predicate.pointer := ipointer;
-           Predicate.iargs := iargs |}
-        oloc (* unused *)
-        ((
-                (* output predicate *)
-                {| Predicate.name:=oname; Predicate.pointer:=opointer; Predicate.iargs:=oargs |},
-                  out
-              ), lines (* unused *)
-         )
-      )
-
+      (* sutuation (unused) *)
+      err 
+      (* input predicate *)
+      {| Predicate.name := Request.Owned (SCtypes.Array (SCtypes.Integer ity, isize)) iinit;
+        Predicate.pointer := ipointer;
+        Predicate.iargs := iargs 
+      |}
+      (* output predicate *)
+      ({| Predicate.name:=oname; Predicate.pointer:=opointer; Predicate.iargs:=oargs |}, out)
+      (* steps *)
+      steps
       (* output context *)
       {|
         Context.computational := ocomputational;
@@ -299,9 +852,138 @@ Inductive log_entry_valid : log_entry -> Prop :=
         Context.constraints := oconstraints;
         Context.global := oglobal
       |}
-    ).
+    )
 
+(* struct case: struct resource is removed from input context *)
+| struct_resource_inference_step:
+  forall isym iinit ipointer iargs
+    oname opointer oargs
+    err out
+    icomputational ilogical iresources iconstraints iglobal
+    ocomputational ological oresources oconstraints oglobal
+    steps,
 
+  (* The following parts of context are not changed *)
+  icomputational = ocomputational ->
+  iglobal = oglobal ->
+  ilogical = ological ->
+  iconstraints = oconstraints ->
+
+  let in_res := ctx_resources_set iresources in
+  let out_res := ctx_resources_set oresources in
+
+  let iname := Request.Owned (SCtypes.Struct isym) iinit in
+
+  iname = oname ->
+  ipointer = opointer ->
+  iargs = oargs ->
+
+  (* Find the struct resource and its fields *)
+  (exists (field_res: ResSet.t),
+      (* The struct unfolds to field resources *)
+      unfold_all iglobal
+        (ResSet.singleton
+          (Request.P {| Predicate.name := iname;
+                       Predicate.pointer := ipointer;
+                       Predicate.iargs := iargs |}, out))
+        field_res /\
+      (* Output context is input context minus all field resources *)
+      ResSet.Equal out_res (ResSet.diff in_res field_res)
+  ) ->
+ 
+  log_entry_valid
+    (PredicateRequest
+      (* input context *)
+      {|
+        Context.computational := icomputational;
+        Context.logical := ilogical;
+        Context.resources := iresources;
+        Context.constraints := iconstraints;
+        Context.global := iglobal
+      |}  
+      (* sutuation (unused) *)
+      err 
+      (* input predicate *)
+      {| Predicate.name := Request.Owned (SCtypes.Struct isym) iinit;
+        Predicate.pointer := ipointer;
+        Predicate.iargs := iargs 
+      |}
+      (* output predicate *)
+      ({| Predicate.name:=oname; Predicate.pointer:=opointer; Predicate.iargs:=oargs |}, out)
+      (* steps *)
+      steps
+      (* output context *)
+      {|
+        Context.computational := ocomputational;
+        Context.logical := ological;
+        Context.resources := oresources;
+        Context.constraints := oconstraints;
+        Context.global := oglobal
+      |}
+  )
+
+(* simple case: non-recursive request, no packing *)
+| simple_resource_inference_step:
+  forall iname  ipointer  iargs
+    oname  opointer  oargs
+    err out
+    icomputational ilogical iresources iconstraints iglobal
+    ocomputational ological oresources oconstraints oglobal
+    steps,
+
+  (* The following parts of context are not changed *)
+  icomputational = ocomputational ->
+  iglobal = oglobal ->
+  ilogical = ological ->
+  iconstraints = oconstraints ->
+
+  let in_res := ctx_resources_set iresources in
+  let out_res := ctx_resources_set oresources in
+
+  iname = oname ->
+  ipointer = opointer ->
+  iargs = oargs ->
+
+  (* [out_res] is a subset of [in_res] with exactly one element [used] removed. *)
+  (exists (upred: Request.Predicate.t),
+      ResSet.Equal (Resource.ResSet.add (P upred, out) out_res) in_res /\
+      (* name matches *)
+      Request.subsumed iname upred.(Request.Predicate.name) /\
+      (* alloc_id matches *)
+      (ptr_alloc_id_eq iglobal iconstraints ipointer upred.(Request.Predicate.pointer)) /\
+      (* pointer and arguments match *)
+      (ptr_addr_and_args_eq iglobal iconstraints ipointer upred.(Request.Predicate.pointer) iargs upred.(Request.Predicate.iargs))
+  )
+
+  ->
+
+    log_entry_valid
+      (PredicateRequest
+        (* input context *)
+        {|
+          Context.computational := icomputational;
+          Context.logical := ilogical;
+          Context.resources := iresources;
+          Context.constraints := iconstraints;
+          Context.global := iglobal
+        |}
+        (* sutuation (unused) *)
+        err 
+        (* input predicate *)
+        {| Predicate.name:=iname; Predicate.pointer:=ipointer; Predicate.iargs:=iargs |}
+        (* output predicate *)
+        ({| Predicate.name:=oname; Predicate.pointer:=opointer; Predicate.iargs:=oargs |}, out)
+        (* steps *)
+        steps
+        (* output context *)
+        {|
+          Context.computational := ocomputational;
+          Context.logical := ological;
+          Context.resources := oresources;
+          Context.constraints := oconstraints;
+          Context.global := oglobal
+        |}
+      ).
 
 (** Proof log is valid if all entries are valid *)
 Definition prooflog_valid (l:Prooflog.log) := List.Forall log_entry_valid l.
