coq/Reasoning/ProofAutomation.v
@@ -1,4 +1,4 @@
-From Ltac2 Require Import Ltac1 Ltac2 Notations Std Constr Env Ident.
+From Ltac2 Require Import Ltac1 Ltac2 Notations Std Constr Env Ident FSet FMap.
  
 From Cn Require Import Prooflog Request Resource Context.
 Require Import Ltac2Utils ResourceInference.
@@ -12,8 +12,8 @@ Ltac2 verbose_msg msg :=
   else
     ().
 
-Ltac2 verbose_print (msg : string) :=
-  verbose_msg (Message.of_string msg).
+Ltac2 verbose_print (s : string) :=
+  verbose_msg (Message.of_string s).
 
 Ltac2 verbose_print_constr (msg:string) (c : constr) :=
   verbose_msg (Message.concat (Message.of_string msg) (Message.of_constr c)).
@@ -46,10 +46,10 @@ Qed.
      Control.throw (Tactic_failure (Some (Message.of_string "Term is not an application (and thus not a P)")))
  end.
   
- Ltac2 res_set_remove_step () :=
+ Ltac2 prove_simple_resource_inference_step () :=
    match! goal with
    | [ |- exists upred,
-       ResSet.Equal (ResSet.add (P upred, ?out) (set_from_list ?out_res)) (set_from_list ?in_res) /\ subsumed _ (Predicate.name upred) ] =>
+       ResSet.Equal (ResSet.add (P upred, ?out) (set_from_list ?out_res)) (set_from_list ?in_res) /\ subsumed _ (Predicate.name upred) /\ _ /\ _ ] =>
      (* break down goal into components *)
      let outname   := Fresh.in_goal @out in
      let inresname := Fresh.in_goal @in_res in
@@ -66,58 +66,138 @@ Qed.
      match diff with
      | [res] =>
          (* single resource [res] matched, extract request as [req] *)
-         let (req,out') := destruct_pair res in
+         let (req,_) := destruct_pair res in
          let p := predicate_of_request req in
          exists $p;
          Std.split false NoBindings;
          (* ResSet subset proof *)
          Control.focus 1 1 (fun () => ltac1:(subst;cbn;ResSetDecide.fsetdec));
-         (* Second subgoal - subsumed *)
-         Control.focus 1 1 (fun () => Std.constructor false; Std.reflexivity ())
+         (* subsumed/\pointereq/\iargseq *)
+         Control.focus 1 1 (fun () => 
+          Std.split false NoBindings;         
+          (* subsumed *)
+          Control.focus 1 1 (fun () =>  Std.constructor false; Std.reflexivity ());
+          (* pointereq/\iargseq *)
+          (Control.focus 1 1 (fun () =>
+           Std.split false NoBindings;         
+           Control.focus 1 1 (Control.shelve);  (* TODO: prove alloc_id equality (via provable) *)
+           Control.focus 1 1 (Control.shelve)  (* TODO: prove pointer address and arguments equality (via provable) *)
+         )))
      | [] =>
          Control.throw (Tactic_failure (Some (Message.of_string "No resource change between the input and output")))
-         (* 
-         Message.print (Message.of_string "Warning: No resource change between the input and output");
-         Control.shelve ()
-         *)
      | _ =>
-         (* Control.throw (Tactic_failure (Some (Message.of_string "More than one resource change between the input and output"))); *)
-         let n := List.length diff in
-         let msg := Message.concat (Message.of_string "Warning: multiple resources changed: ") (Message.of_int n) in
-         Message.print msg;
-         (if verbose then
-            verbose_print_constr "Combined output" out ;
-            (* Print changed resources: *)
-            let print_resource res :=
-              Message.print (Message.of_constr res)
-            in
-            List.iter print_resource diff
-          else ());
-         Control.shelve ()
+         Control.throw (Tactic_failure (Some (Message.of_string "More than one resource change between the input and output")))
      end
- end.
+   | [ |- _ ] => Control.throw (Tactic_failure (Some (Message.of_string "prove_simple_resource_inference_step: match failed")))
+   end.
 
-Ltac2 prove_unfold_step () :=
+
+(* [struct_resource_inference_step] constructor pre-condition proof *)
+ Ltac2 prove_struct_resource_inference_step () :=
+ match! goal with
+ | [ |- exists field_res,
+        unfold_all _ _ field_res /\
+        ResSet.Equal (set_from_list ?out_res) (ResSet.diff (set_from_list ?in_res) field_res) ] =>
+
+   (* now try to compute field_res from in_res and out_res *)
+   let list_of_constr l := destruct_list (constr:(Resource.t)) l in
+   let in_res_list  := list_of_constr  in_res in
+   let out_res_list := list_of_constr out_res in
+   let field_res := const_list_subtract in_res_list out_res_list in
+   if List.is_empty field_res then
+    Control.throw (Tactic_failure (Some (Message.of_string "No resource change between the input and output")))
+   else
+     let cfield_res := recons_list (constr:(Resource.t)) field_res in
+     let field_res_set := constr:(set_from_list $cfield_res) in
+     exists $field_res_set;
+     Std.split false NoBindings;
+     Control.focus 1 1 (fun () =>
+      (* Proof using computational reflection: *)
+      Control.shelve ()
+     );  (* unfold predicate *)
+     Control.focus 1 1 (fun () =>
+      pairwise_decidability (constr:(Resource_as_MiniDecidableType.eq_dec)) in_res_list ;
+      ltac1:(cbn;ResSetDecide.fsetdec)
+     )
+ | [ |- _ ] => Control.throw (Tactic_failure (Some (Message.of_string "prove_struct_resource_inference_step: match failed")))
+end.
+
+Ltac2 prove_unfold_step (hints:constr) :=
   match! goal with
-  | [ |- unfold_step ?c ?c' ] =>
+  | [ |- unfold_step _ _ ] =>
       Std.constructor false;
       Control.focus 1 1 (fun () => Std.reflexivity ());
       Control.focus 1 1 (fun () => Std.reflexivity ());
       Control.focus 1 1 (fun () => Std.reflexivity ());
       Control.focus 1 1 (fun () => Std.reflexivity ());
 
-      Message.print (Message.of_string "TODO: Shelving unfold step pre-condition.");
-      Control.shelve ()
-
+      (* Proof using computational reflection: *)
+      ltac1:(hints |- apply unfold_all_explicit_eq with (unfold_changed := (unfold_step_flatten hints))) 
+        (Ltac1.of_constr hints);
+      ltac1:(apply unfold_all_explicit_fun_eq);
+      ltac1:(vm_compute);
+      ltac1:(reflexivity)
+  | [ |- _ ] => Control.throw (Tactic_failure (Some (Message.of_string "prove_unfold_step: match failed")))
   end.
 
- Ltac2 prove_log_entry_valid () :=
-   match! goal with
-   | [ |- log_entry_valid (ResourceInferenceStep _ (PredicateRequest _ ?p _ _) _) ] =>
+ Ltac2 prove_log_entry_valid n :=
+ let smsg s := Message.concat (Message.concat (Message.of_string "Step #") (Message.of_int n)) (Message.concat (Message.of_string ": ") (Message.of_string s)) in
+ let msg m := Message.concat (Message.concat (Message.of_string "Step #") (Message.of_int n)) (Message.concat (Message.of_string ": ") m) in
+ match! goal with
+    (* PredicateRequest for array *)
+  | [ |- log_entry_valid (PredicateRequest _ _ 
+      {| 
+        Predicate.name := Request.Owned (SCtypes.Array _) _;
+        Predicate.pointer := _; Predicate.iargs := _ 
+      |}
+      _ _ _) ] =>
+        Message.print (msg (Message.of_string "Arrays are not supported yet"));
+        Std.constructor_n false 2 NoBindings (* apply array_resource_inference_step *)
+    (* PredicateRequest for struct *)
+  | [ |- log_entry_valid (PredicateRequest _ ?s
+      {| 
+        Predicate.name := Request.Owned (SCtypes.Struct ?isym) _;
+        Predicate.pointer := _; Predicate.iargs := _ 
+      |}
+      _ ?hints _) ] =>
+       verbose_msg (smsg "Checking PredicateRequest for Struct");
+       verbose_print_constr "    Situation: " s;
+       verbose_print_constr "    Predicate symbol name: " isym;
+       let lhints := destruct_list (constr:(log_entry)) hints in
+       verbose_msg (Message.concat (Message.of_string "    Number of hints: ") (Message.of_int (List.length lhints)));
+       Std.constructor_n false 3 NoBindings; (* apply struct_resource_inference_step *)
+       Control.focus 1 1 (fun () => Std.reflexivity ());
+       Control.focus 1 1 (fun () => Std.reflexivity ());
+       Control.focus 1 1 (fun () => Std.reflexivity ());
+       Control.focus 1 1 (fun () => Std.reflexivity ());
+       Control.focus 1 1 (fun () => Std.reflexivity ());
+       Control.focus 1 1 (fun () => Std.reflexivity ());
+       Control.focus 1 1 (fun () => Std.reflexivity ());
+       Control.focus 1 1 (fun () => 
+        let clause := { on_hyps := None; on_concl := AllOccurrences } in
+          Std.unfold [(const_to_const_reference constr:(@ctx_resources_set), AllOccurrences)] clause;
+          Std.cbn 
+          { rStrength := Std.Norm;
+            rBeta := true;
+            rMatch := true;
+            rFix := true;
+            rCofix := true;
+            rZeta := true;
+            rDelta := true;
+            rConst := [const_to_const_reference constr:(@set_from_list); const_to_const_reference constr:(@Sym.map_from_list)]
+          } clause ;
+          prove_struct_resource_inference_step ()
+       )
+    (* PredicateRequest for non-Struct *)
+  | [ |- log_entry_valid (PredicateRequest _ ?s ?p _ _ _)] =>
        (* PredicateRequest case *)
-       verbose_print "Checking PredicateRequest";
+       verbose_msg (smsg "Checking PredicateRequest for non-Struct");
+       verbose_print_constr "    Situation: " s;
        verbose_print_constr "    Predicate: " p;
-       Std.constructor false;
+       Std.constructor false; (* apply simple_resource_inference_step*)
+       Control.focus 1 1 (fun () => Std.reflexivity ());
+       Control.focus 1 1 (fun () => Std.reflexivity ());
+       Control.focus 1 1 (fun () => Std.reflexivity ());
        Control.focus 1 1 (fun () => Std.reflexivity ());
        Control.focus 1 1 (fun () => Std.reflexivity ());
        Control.focus 1 1 (fun () => Std.reflexivity ());
@@ -135,19 +215,24 @@ Ltac2 prove_unfold_step () :=
              rDelta := true;
              rConst := [const_to_const_reference  constr:(@set_from_list)]
            } clause ;
-         res_set_remove_step ()
+           prove_simple_resource_inference_step ()
        )
-   | [ |- log_entry_valid (ResourceInferenceStep _ (UnfoldResources _) _) ] =>
-      (* UnfoldResources case *)
-      verbose_print "Checking UnfoldResources";
+    (* UnfoldResources step *)
+  | [ |- log_entry_valid (UnfoldResources _ _ ?hints _) ] =>
+      verbose_msg (smsg "Checking UnfoldResources");
+      let lhints := destruct_list (constr:(log_entry)) hints in
+      verbose_msg (Message.concat (Message.of_string "    Number of hints: ") (Message.of_int (List.length lhints)));
       Std.constructor false;
-      prove_unfold_step ()
-   end.
- 
+      prove_unfold_step hints
+  | [ |- _ ] => 
+      Control.throw (Tactic_failure (Some (msg (Message.of_string "prove_log_entry_valid: match failed"))))
+  end.
+
+ (* Attempts to prove that all log entries in the list are valid *)
  Ltac2 prove_log_entry_list_valid () :=
    match! goal with
    | [ |- List.Forall log_entry_valid ?l ] =>
-       let rec aux l :=
+       let rec aux n l :=
          let nil_constr := constr:(@nil log_entry) in
          let cons_constr := constr:(@cons log_entry) in
          match Constr.Unsafe.kind l with
@@ -159,18 +244,16 @@ Ltac2 prove_unfold_step () :=
                (* nil case *)
                Std.constructor false
              else if Constr.equal f_name cons_name then
-               (* cons case *)
-               let head := Array.get args 1 in
                let tail := Array.get args 2 in
                Std.constructor false;
-               Control.focus 1 1 (fun () => prove_log_entry_valid ());
-               Control.focus 1 1 (fun () => aux tail)
+               Control.focus 1 1 (fun () => prove_log_entry_valid n);
+               Control.focus 1 1 (fun () => aux (Int.add n 1) tail)
              else
                Control.throw (Tactic_failure (Some (Message.of_string "Not a list")))
          | _ =>
              Control.throw (Tactic_failure (Some (Message.of_string "Not a list")))
          end
-       in aux l
+       in aux 0 l
    end.
  
  
