tests/run-cn-coq.sh
@@ -1,10 +1,10 @@
 #!/usr/bin/env bash
 
 # CI test for CN Coq extraction.
-# OPAM package `cn-coq` must be installed.
+# If running without -d flag, OPAM package `cn-coq` must be installed.
+# If running with -d flag, it must be run from the root of the Cn repository.
 
 set -uo pipefail
-
 
 # List of blacklisted files that are known to run out of memory in Coq.
 # Paths must be relative to the 'tests/cn' directory.
@@ -12,9 +12,11 @@ set -uo pipefail
 BLACKLISTED_FILES=(
     tree16/as_partial_map/tree16.c
     tree16/as_mutual_dt/tree16.c
+    append.c
     mergesort.c
     mergesort_alt.c
     mutual_rec/mutual_rec2.c
+    mutual_rec/mutual_rec3.c    
 )
 
 # Parse command line options
@@ -25,7 +27,7 @@ USE_DUNE=0
 COQ_PROOF_LOG=0
 COQ_CHECK_PROOF_LOG=0
 
-while getopts "dpef: v" opt; do
+while getopts "dpcef: v" opt; do
     case ${opt} in
         d)
             USE_DUNE=1
@@ -47,12 +49,12 @@ while getopts "dpef: v" opt; do
             VERBOSE_USAGE=1
             ;;
         *)
-            echo "Usage: $0 [-e] [-f file] [-v]"
+            echo "Usage: $0 [-e] [-d] [-p] [-c] [-v] [-f file]"
             echo "  -e  Stop on error and preserve temporary directory"
             echo "  -f  Run single test file (implies -e)"
             echo "  -d  Use dune to run CN"
             echo "  -p  Include proof log in Coq export"
-            echo "  -c  Check proof log in Coq export"
+            echo "  -c  Run proof automation on proof log"
             echo "  -v  Verbose output for resource usage logging"
             exit 1
             ;;
@@ -84,9 +86,9 @@ PASSED_COUNT=0
 FAILED_COUNT=0
 
 if [ ${USE_DUNE} -eq 1 ]; then
-    CN=(${WITH_CN:=dune exec cn --})
+    CN=(${WITH_CN:=dune exec -p cn,cn-coq cn --})
     unset CERB_INSTALL_PREFIX
-    COQ_CN_THEORIES_DIR="$(realpath "../_build/default/coq")"
+    COQ_CN_THEORIES_DIR="$(realpath "_build/default/coq")"
     COQ_MAKEFILE_FLAGS="-R . Top -R ${COQ_CN_THEORIES_DIR}/Cerberus/ Cerberus -R ${COQ_CN_THEORIES_DIR}/Cn/ Cn -R ${COQ_CN_THEORIES_DIR}/Reasoning/ Reasoning"
 else
     CN=(cn)
